VHDL_Hoare_Complete.thy
@@ -1,0 +1,1811 @@
+(*
+ * Copyright 2019, NTU
+ *
+ * This software may be distributed and modified according to the terms of
+ * the BSD 2-Clause license. Note that NO WARRANTY is provided.
+ * See "LICENSE_BSD2.txt" for details.
+ *
+ *  Author: Albert Rizaldi, NTU Singapore
+ *)
+
+theory VHDL_Hoare_Complete
+  imports Femto_VHDL VHDL_Hoare
+begin
+
+subsection "A sound and complete Hoare logic for VHDL's sequential statements"
+
+text \<open>This theory is the second attempt for defining a Hoare logic for VHDL's sequential statement. 
+As shown in the very last part of this theory, we prove that this definition is both sound and 
+complete.\<close>
+
+typedef (overloaded) ('signal) worldline2 = 
+  "{w :: 'signal worldline . (\<exists>t. \<forall>t'. t' > t \<longrightarrow> (\<lambda>s. w s t') = (\<lambda>s. w s t))}" 
+  morphisms Rep_worldline Abs_worldline
+proof -
+  define wit :: "'signal worldline" where "wit \<equiv> (\<lambda>s t. False)"
+  hence "\<forall>t'. t' > 0 \<longrightarrow> (\<lambda>s. wit s t') = (\<lambda>s. wit s 0)"
+    by auto
+  thus ?thesis
+    by (auto intro: exI[where x="wit"])
+qed
+
+setup_lifting type_definition_worldline2
+
+text \<open> The reason why the first attempt of defining the semantics in @{theory Draft.VHDL_Hoare} is 
+not complete is because not all worldline can be transformed into elements of the operational 
+semantics, especially the transaction @{term "\<tau> :: 'signal transaction"}. Why is this so?
+
+Imagine a worldline @{term "w"} where it always alternate between @{term "True :: val"} and @{term
+"False :: val"} for a specific signal @{term "sig :: 'signal"}. When we attempt to find the
+derivative via @{term "derivative_raw w"}, its result cannot be a @{typ "'signal transaction"}
+because it will have infinite mappings (since it constantly changes the value between @{term "True
+:: val"} and @{term "False :: val"}, and a @{typ "'signal transaction"} needs to be zero at nearly
+everywhere, i.e., eventually the mapping will ``die out''.
+
+The typedef of @{typ "'signal worldline2"} imposes that eventually there will be no more mapping. 
+Hence, when we attempt to find its derivative, we can construct a @{typ "'signal transaction"}.
+\<close>
+
+definition worldline_deg :: "'signal worldline2 \<Rightarrow> nat" where
+  "worldline_deg w = (LEAST n. \<forall>t > n. \<forall>s. Rep_worldline w s t = Rep_worldline w s n)"
+
+lemma existence_of_degree:
+  fixes w :: "'signal worldline2"
+  shows "\<exists>x. \<forall>t > x. \<forall>s. Rep_worldline w s t = Rep_worldline w s x" 
+  by transfer meson
+
+lemma property_of_degree:
+  fixes w :: "'signal worldline2"
+  defines "d \<equiv> worldline_deg w"
+  shows "\<forall>t > d. \<forall>s. Rep_worldline w s t = Rep_worldline w s d"
+  using LeastI_ex[OF existence_of_degree] unfolding d_def worldline_deg_def by auto
+
+lift_definition worldline_upd2 :: 
+  "'signal worldline2 \<Rightarrow> 'signal \<Rightarrow> nat \<Rightarrow> val \<Rightarrow> 'signal worldline2" ("_[_, _:=\<^sub>2 _]")
+  is worldline_upd
+proof -
+  fix w :: "'signal \<Rightarrow> nat \<Rightarrow> val" 
+  fix sig v
+  fix t :: nat
+  assume "\<exists>t. \<forall>t'>t. (\<lambda>s'. w s' t') = (\<lambda>s'. w s' t)"
+  then obtain tcurr :: "nat" where *: "\<forall>t' > tcurr. (\<lambda>s'. w s' t') = (\<lambda>s'. w s' tcurr)"
+    by auto
+  have "t < tcurr \<or> tcurr \<le> t"
+    by auto
+  moreover
+  { assume "t < tcurr"
+    hence "\<forall>t'> tcurr. (\<lambda>s. w[sig, t:= v] s t') = (\<lambda>s. w[sig, t:= v] s tcurr)"
+      by (metis * less_trans not_less_iff_gr_or_eq worldline_upd_def)
+    hence "\<exists>t''. \<forall>t'> t''. (\<lambda>s. w[sig, t:= v] s t') = (\<lambda>s. w[sig, t:= v] s t'')"
+      by auto }
+  moreover
+  { assume "tcurr \<le> t"
+    hence "\<forall>t'> t. (\<lambda>s. w[sig, t:= v] s t') = (\<lambda>s. w[sig, t:= v] s t)"
+      by (metis (full_types) "*" le_less_trans nat_less_le worldline_upd_def)
+    hence "\<exists>t''. \<forall>t'> t''. (\<lambda>s. w[sig, t:= v] s t') = (\<lambda>s. w[sig, t:= v] s t'')"
+      by auto }
+  ultimately show "\<exists>t''. \<forall>t'>t''. (\<lambda>s. w[sig, t:= v] s t') = (\<lambda>s. w[sig, t:= v] s t'')"
+    by auto
+qed
+        
+lift_definition worldline_inert_upd2 :: 
+  "'signal worldline2 \<Rightarrow> 'signal \<Rightarrow> nat \<Rightarrow> nat \<Rightarrow> val \<Rightarrow> 'signal worldline2" ("_[_, _, _ :=\<^sub>2 _]")
+  is worldline_inert_upd 
+proof -
+  fix w :: "'signal \<Rightarrow> nat \<Rightarrow> val" 
+  fix sig v
+  fix t1 t2 :: nat  
+  assume "\<exists>t. \<forall>t'>t. (\<lambda>s'. w s' t') = (\<lambda>s'. w s' t)"
+  then obtain tcurr :: "nat" where *: "\<forall>t' > tcurr. (\<lambda>s'. w s' t') = (\<lambda>s'. w s' tcurr)"
+    by auto
+  have "t1 + t2 < tcurr \<or> tcurr \<le> t1 + t2"
+    by auto  
+  moreover
+  { assume "t1 + t2 < tcurr"
+    hence "\<forall>t'> tcurr. (\<lambda>s. w[sig, t1, t2 := v] s t') = (\<lambda>s. w[sig, t1, t2 := v] s tcurr)"
+      by (metis "*" le_add1 le_less_trans less_irrefl_nat order.strict_trans  worldline_inert_upd_def)
+    hence "\<exists>t''. \<forall>t'> t''. (\<lambda>s. w[sig, t1, t2:= v] s t') = (\<lambda>s. w[sig, t1, t2:= v] s t'')"
+      by auto }    
+  moreover
+  { assume "tcurr \<le> t1 + t2"
+    have "\<forall>t'> t1 + t2. (\<lambda>s. w[sig, t1, t2 := v] s t') = (\<lambda>s. w[sig, t1, t2 := v] s (t1 + t2))"
+    proof (rule, rule)
+      fix t'
+      assume "t' > t1 + t2" hence "t' > tcurr" using `t1 + t2 \<ge> tcurr` by auto
+      { fix s
+        have "s \<noteq> sig \<or> s = sig" by auto
+        moreover
+        { assume "s \<noteq> sig"
+          hence "w[sig, t1, t2:= v] s t' = w[sig, t1, t2 := v] s (t1 + t2)"
+            by (metis "*" \<open>tcurr < t'\<close> \<open>tcurr \<le> t1 + t2\<close> le_less option.sel worldline_inert_upd_def) }
+        moreover
+        { assume "s = sig"
+          hence "w[sig, t1, t2 := v] s t' = w[sig, t1, t2 := v] s (t1 + t2)"
+            by (metis \<open>t1 + t2 < t'\<close> not_less_iff_gr_or_eq trans_less_add1 worldline_inert_upd_def) }
+        ultimately have "w[sig, t1, t2 := v] s t' = w[sig, t1, t2 := v] s (t1 + t2)"
+          by auto }
+      thus " (\<lambda>s. w[sig, t1, t2 := v] s t') = (\<lambda>s. w[sig, t1, t2 := v] s (t1 + t2))"
+        by auto
+    qed
+    hence "\<exists>t''. \<forall>t'> t''. (\<lambda>s. w[sig, t1, t2:= v] s t') = (\<lambda>s. w[sig, t1, t2:= v] s t'')"
+      by auto }   
+  ultimately show "\<exists>t''. \<forall>t'> t''. (\<lambda>s. w[sig, t1, t2:= v] s t') = (\<lambda>s. w[sig, t1, t2:= v] s t'')"
+    by auto 
+qed
+
+lift_definition state_of_world2 :: "'signal worldline2 \<Rightarrow> nat \<Rightarrow> 'signal state" is
+  state_of_world .
+
+lift_definition event_of_world2 :: "'signal worldline2 \<Rightarrow> nat \<Rightarrow> 'signal event" is
+  event_of_world .
+
+lift_definition beh_of_world2 :: "'signal worldline2 \<Rightarrow> nat \<Rightarrow> 'signal transaction" is 
+  beh_of_world_raw  unfolding beh_of_world_raw_def zero_map by auto
+
+lemma [simp]:
+  "beh_of_world2 w 0 = 0"
+  by (transfer', auto simp add:  beh_of_world_raw_def zero_option_def zero_fun_def)
+
+lift_definition beval_world2 :: "'signal worldline2 \<Rightarrow> nat \<Rightarrow> 'signal bexp \<Rightarrow> val" 
+  is beval_world .
+
+type_synonym 'signal assn2 = "'signal worldline2 \<Rightarrow> bool"
+
+inductive
+  seq_hoare2 :: "nat \<Rightarrow> 'signal assn2 \<Rightarrow> 'signal seq_stmt \<Rightarrow> 'signal assn2 \<Rightarrow> bool" ("\<turnstile>\<^sub>_ ([(1_)]/ (_)/ [(1_)])" 50)
+  where
+Null2: "\<turnstile>\<^sub>t [P] Bnull [P]" |
+Assign2: "\<turnstile>\<^sub>t [\<lambda>w. P(w[sig, t + dly :=\<^sub>2 beval_world2 w t exp])] Bassign_trans sig exp dly [P]" |
+
+AssignI2: "\<turnstile>\<^sub>t [\<lambda>w. P(w[sig, t, dly :=\<^sub>2 beval_world2 w t exp])] Bassign_inert sig exp dly [P]" |
+
+Comp2: "\<lbrakk> \<turnstile>\<^sub>t [P] s1 [Q]; \<turnstile>\<^sub>t [Q] s2 [R]\<rbrakk> \<Longrightarrow> \<turnstile>\<^sub>t [P] Bcomp s1 s2 [R]" |
+
+If2: "\<lbrakk>\<turnstile>\<^sub>t [\<lambda>w. P w \<and> beval_world2 w t g] s1 [Q]; \<turnstile>\<^sub>t [\<lambda>w. P w \<and> \<not> beval_world2 w t  g] s2 [Q]\<rbrakk>
+        \<Longrightarrow>  \<turnstile>\<^sub>t [P] Bguarded g s1 s2 [Q]" |
+
+Conseq2: "\<lbrakk>\<forall>w. P' w \<longrightarrow> P w; \<turnstile>\<^sub>t [P] s [Q]; \<forall>w. Q w \<longrightarrow> Q' w\<rbrakk> \<Longrightarrow> \<turnstile>\<^sub>t [P'] s [Q']"
+
+inductive_cases seq_hoare2_ic: "\<turnstile>\<^sub>t [P] s [Q]"
+
+lemma BnullE_hoare2:
+  assumes "\<turnstile>\<^sub>t [P] s [Q]"
+  assumes "s = Bnull"
+  shows "\<forall>w. P w \<longrightarrow> Q w"
+  using assms
+  by (induction rule:seq_hoare2.induct, auto)
+
+lemma BnullE'_hoare2:
+  "\<turnstile>\<^sub>t [P] Bnull [Q] \<Longrightarrow> \<forall>w. P w \<longrightarrow> Q w"
+  using BnullE_hoare2 by blast
+
+lemma BassignE_hoare2:
+  assumes "\<turnstile>\<^sub>t [P] s [Q]"
+  assumes "s = Bassign_trans sig exp dly"
+  shows "\<forall>w. P w \<longrightarrow> Q(w[sig, t + dly :=\<^sub>2 beval_world2 w t exp])"
+  using assms
+  by (induction rule: seq_hoare2.induct, auto)
+
+lemma Bassign_inertE_hoare2:
+  assumes "\<turnstile>\<^sub>t [P] s [Q]"
+  assumes "s = Bassign_inert sig exp dly"
+  shows "\<forall>w. P w \<longrightarrow> Q(w[sig, t, dly :=\<^sub>2 beval_world2 w t exp])"
+  using assms
+  by (induction rule: seq_hoare2.induct, auto)
+
+lemma BcompE_hoare2:
+  assumes "\<turnstile>\<^sub>t [P] s [R]"
+  assumes "s = Bcomp s1 s2"
+  shows "\<exists>Q. \<turnstile>\<^sub>t [P] s1 [Q] \<and> \<turnstile>\<^sub>t [Q] s2 [R]"
+  using assms Conseq2
+  by (induction rule:seq_hoare2.induct, auto) (blast)
+
+lemmas [simp] = seq_hoare2.Null2 seq_hoare2.Assign2 seq_hoare2.Comp2 seq_hoare2.If2
+lemmas [intro!] = seq_hoare2.Null2 seq_hoare2.Assign2 seq_hoare2.Comp2 seq_hoare2.If2
+
+lemma strengthen_pre_hoare2:
+  assumes "\<forall>w. P' w \<longrightarrow> P w" and "\<turnstile>\<^sub>t [P] s [Q]"
+  shows "\<turnstile>\<^sub>t [P'] s [Q]"
+  using assms by (blast intro: Conseq2)
+
+lemma weaken_post_hoare2:
+  assumes "\<forall>w. Q w \<longrightarrow> Q' w" and "\<turnstile>\<^sub>t [P] s [Q]"
+  shows "\<turnstile>\<^sub>t [P] s [Q']"
+  using assms by (blast intro: Conseq2)
+
+lemma Assign'_hoare2:
+  assumes "\<forall>w. P w \<longrightarrow> Q (worldline_upd2 w sig (t + dly) (beval_world2 w t exp))"
+  shows "\<turnstile>\<^sub>t [P] Bassign_trans sig exp dly [Q]"
+  using assms by (simp add: strengthen_pre_hoare2)
+
+subsection \<open>Validity of Hoare proof rules\<close>
+
+lift_definition worldline2 :: 
+  "nat \<Rightarrow> 'signal state \<Rightarrow> 'signal transaction \<Rightarrow> 'signal transaction \<Rightarrow> 'signal worldline2" 
+  is worldline
+proof -
+  fix t0 :: nat
+  fix \<sigma> :: "'signal state"
+  fix \<theta> \<tau> :: "'signal transaction"
+
+  define last where "last \<equiv> max (Poly_Mapping.degree \<tau>) (Poly_Mapping.degree \<theta>)"
+
+  have "\<forall>t'>max last t0. (\<lambda>s. worldline t0 \<sigma> \<theta> \<tau> s t') = (\<lambda>s. worldline t0 \<sigma> \<theta> \<tau> s (max last t0))"
+  proof (rule, rule)
+    fix t'
+    assume "max last t0 < t'"
+    { fix s
+      have *: "\<And>n. max last t0 < n \<Longrightarrow> n \<le> t' \<Longrightarrow> lookup \<tau> n = 0"
+        by (simp add: beyond_degree_lookup_zero local.last_def)          
+      have "worldline t0 \<sigma> \<theta> \<tau> s t' = signal_of2 (\<sigma> s) \<tau> s t'"
+        by (meson \<open>max last t0 < t'\<close> less_imp_not_less less_max_iff_disj worldline_def)
+      also have "... = signal_of2 (\<sigma> s) \<tau> s (max last t0)"
+        using signal_of2_less_ind[OF * `max last t0 < t'`] by metis
+      also have "... = worldline t0 \<sigma> \<theta> \<tau> s (max last t0)"
+        by (simp add: worldline_def)
+      finally have "worldline t0 \<sigma> \<theta> \<tau> s t' = worldline t0 \<sigma> \<theta> \<tau> s (max last t0)"
+        by auto }
+    thus "(\<lambda>s. worldline t0 \<sigma> \<theta> \<tau> s t') = (\<lambda>s. worldline t0 \<sigma> \<theta> \<tau> s (max last t0))"
+      by auto
+  qed
+  thus "\<exists>t''. \<forall>t'>t''. (\<lambda>s. worldline t0 \<sigma> \<theta> \<tau> s t') = (\<lambda>s. worldline t0 \<sigma> \<theta> \<tau> s t'')"
+    by (auto intro:exI[where x="max last t0"])
+qed
+
+definition difference :: "'signal worldline2 \<Rightarrow> nat \<Rightarrow> 'signal \<rightharpoonup> val" where
+  "difference w t = (\<lambda>s. if Rep_worldline w s t \<noteq> Rep_worldline w s (t - 1) then Some (Rep_worldline w s t) else None)"
+
+lemma difference_beyond_degree:
+  fixes w :: "'signal worldline2"
+  defines "d \<equiv> worldline_deg w"
+  shows "\<forall>n > d. difference w n = 0"
+proof -
+  { fix s
+    have "\<forall>n > d. Rep_worldline w s n = Rep_worldline w s d"
+      using property_of_degree unfolding d_def by auto
+    hence "\<forall>n > d. Rep_worldline w s n = Rep_worldline w s (n - 1)"
+      by (metis (full_types) diff_Suc_1 gr0_implies_Suc less_add_same_cancel2 less_imp_Suc_add 
+      less_linear not_add_less1 trans_less_add1) }
+  thus ?thesis
+    unfolding difference_def unfolding zero_fun_def by (simp add: zero_option_def)
+qed
+
+lift_definition derivative :: "'signal worldline2 \<Rightarrow> nat \<Rightarrow> 'signal transaction" 
+  is "\<lambda>w t n. if n < t then Map.empty else if n = t then Some o (\<lambda>s. Rep_worldline w s t) else difference w n"
+  unfolding sym[OF eventually_cofinite] MOST_nat
+proof -
+  fix w :: "'signal worldline2"
+  fix t :: nat
+  define d where "d = worldline_deg w"
+  have "\<forall>n > max d t. difference w n = 0"
+    by (simp add: d_def difference_beyond_degree)
+  hence "\<forall>n>max d t. (if n < t then Map.empty else if n = t then Some \<circ> (\<lambda>s. Rep_worldline w s t) else difference w n) = 0"
+    by auto
+  thus "\<exists>t''. \<forall>n>t''. (if n < t then Map.empty else if n = t then Some \<circ> (\<lambda>s. Rep_worldline w s t) else difference w n) = 0"
+    by blast
+qed
+
+definition destruct_worldline :: 
+  "'signal worldline2 \<Rightarrow> nat \<Rightarrow> ('signal state \<times> 'signal event \<times> 'signal transaction \<times> 'signal transaction)" 
+  where
+  "destruct_worldline w t = (let \<sigma> = (\<lambda>s. Rep_worldline w s t); 
+                                 \<theta> = poly_mapping_of_fun (\<lambda>t. Some o (\<lambda>s. (Rep_worldline w) s t)) 0 t;
+                                 \<gamma> = {s. \<sigma> s \<noteq> signal_of2 False \<theta> s (t - 1)}; 
+                                 \<tau> = derivative_raw (Rep_worldline w) (worldline_deg w) t 
+                             in (\<sigma>, \<gamma>, \<theta>, \<tau>))"
+
+lemma destruct_worldline_exist:
+  "\<exists>\<sigma> \<gamma> \<theta> \<tau>. destruct_worldline w t = (\<sigma>, \<gamma>, \<theta>, \<tau>)"
+  unfolding destruct_worldline_def Let_def by auto
+
+lemma worldline2_constructible:
+  fixes w :: "'signal worldline2"
+  assumes "destruct_worldline w t = (\<sigma>, \<gamma>, \<theta>, \<tau>)"
+  shows "w = worldline2 t \<sigma> \<theta> \<tau> \<and> context_invariant t \<sigma> \<gamma> \<theta> \<tau>"
+proof -
+  have "\<exists>t. \<forall>t'>t. (\<lambda>s. Rep_worldline w s t') = (\<lambda>s. Rep_worldline w s t)"
+    by transfer auto
+  thus ?thesis
+    using assms unfolding destruct_worldline_def Let_def worldline_deg_def
+  proof transfer'
+    fix w :: "'signal worldline" 
+    fix t \<sigma> \<gamma> 
+    fix \<theta> \<tau> :: "'signal transaction"
+    assume *: "\<exists>t. \<forall>t'>t. (\<lambda>s. w s t') = (\<lambda>s. w s t)"
+    then obtain d where d_def: "d = (LEAST t. \<forall>t'>t. (\<lambda>s. w s t') = (\<lambda>s. w s t))"
+      by auto
+    have d_prop: "\<forall>t'>d. (\<lambda>s. w s t') = (\<lambda>s. w s d)" 
+      using LeastI_ex[OF *] unfolding d_def  by blast 
+    hence d_prop': "\<And>n s. d < n \<Longrightarrow> w s n = w s d"
+      by meson
+    have d_def': "d = (LEAST n. \<forall>t>n. \<forall>s. w s t = w s n)"
+      unfolding d_def  by metis
+    assume **:
+      "(\<lambda>s. w s t, 
+        {s. w s t \<noteq> signal_of2 False (poly_mapping_of_fun (\<lambda>t. Some \<circ> (\<lambda>s. w s t)) 0 t) s (t - 1)}, 
+        poly_mapping_of_fun (\<lambda>t. Some \<circ> (\<lambda>s. w s t)) 0 t,
+        derivative_raw w (LEAST n. \<forall>t>n. \<forall>s. w s t = w s n) t) = (\<sigma>, \<gamma>, \<theta>, \<tau>)"  
+    hence \<sigma>_def: "\<sigma> = (\<lambda>s. w s t)" and 
+          \<gamma>_def: "\<gamma> = {s. w s t \<noteq> signal_of2 False (poly_mapping_of_fun (\<lambda>t. Some \<circ> (\<lambda>s. w s t)) 0 t) s (t - 1)}" and
+          \<theta>_def: "\<theta> = poly_mapping_of_fun (\<lambda>t. Some \<circ> (\<lambda>s. w s t)) 0 t"
+      by auto
+    have \<tau>_def: "\<tau> = derivative_raw w d t"
+      using ** unfolding d_def' by auto 
+    have "w = worldline t \<sigma> \<theta> \<tau>"
+    proof (rule ext, rule ext, cases "t \<le> d")
+      case True
+      fix s' t' 
+      have "t' < t \<or> t \<le> t'" by auto
+      moreover
+      { assume "t' < t"
+        hence "worldline t \<sigma> \<theta> \<tau> s' t' =  signal_of2 False \<theta> s' t'"
+          unfolding worldline_def by auto
+        also have "... = w s' t'"
+          using signal_of2_poly_mapping_fun[OF `t' < t`] unfolding \<theta>_def by metis
+        finally have "w s' t' = worldline t \<sigma> \<theta> \<tau> s' t'"
+          by auto }
+      moreover
+      { assume "t \<le> t'"
+        hence "worldline t \<sigma> \<theta> \<tau> s' t' = signal_of2 (\<sigma> s') \<tau> s' t'"
+          unfolding worldline_def by auto
+        also have "... = w s' t'"
+          unfolding \<tau>_def using signal_of2_derivative_raw'[OF `t \<le> t'` True] d_prop' by metis
+        finally have "w s' t' = worldline t \<sigma> \<theta> \<tau> s' t'"
+          by auto }
+      ultimately show "w s' t' = worldline t \<sigma> \<theta> \<tau> s' t'"
+        by auto
+    next
+      case False
+      fix s' t' 
+      have "t' < t \<or> t \<le> t'" by auto
+      moreover
+      { assume "t' < t"
+        hence "worldline t \<sigma> \<theta> \<tau> s' t' =  signal_of2 False \<theta> s' t'"
+          unfolding worldline_def by auto
+        also have "... = w s' t'"
+          using signal_of2_poly_mapping_fun[OF `t' < t`] unfolding \<theta>_def by metis
+        finally have "w s' t' = worldline t \<sigma> \<theta> \<tau> s' t'"
+          by auto }
+      moreover
+      { assume "t \<le> t'"
+        hence "worldline t \<sigma> \<theta> \<tau> s' t' = signal_of2 (\<sigma> s') \<tau> s' t'"
+          unfolding worldline_def by auto
+        also have "... = signal_of2 (\<sigma> s') 0 s' t'"
+          unfolding \<tau>_def using derivative_raw_zero False  by (metis le_less_linear)
+        also have "... = \<sigma> s'"
+          using signal_of2_empty by fastforce
+        also have "... = w s' t"
+          unfolding \<sigma>_def by auto
+        also have "... = w s' t'"
+          using d_prop'[of "t"] d_prop'[of "t'"] False `t \<le> t'` by auto
+        finally have "w s' t' = worldline t \<sigma> \<theta> \<tau> s' t'"
+          by auto }
+      ultimately show "w s' t' = worldline t \<sigma> \<theta> \<tau> s' t'"
+        by auto
+    qed
+    have "\<forall>n. t \<le> n \<longrightarrow> lookup \<theta> n = 0"
+      unfolding \<theta>_def apply transfer' by auto
+    moreover have "\<forall>n. n < t \<longrightarrow> lookup \<tau> n = 0"
+      unfolding \<tau>_def 
+      by (transfer', metis (mono_tags) derivative_raw.rep_eq derivative_raw_zero lookup_zero)
+    moreover have "\<forall>s. s \<in> dom (lookup \<tau> t) \<longrightarrow> \<sigma> s = the (lookup \<tau> t s)"
+      unfolding \<tau>_def \<sigma>_def by transfer' auto
+    ultimately have "context_invariant t \<sigma> \<gamma> \<theta> \<tau>"
+      unfolding \<gamma>_def context_invariant_def \<sigma>_def \<theta>_def by auto
+    thus " w = worldline t \<sigma> \<theta> \<tau> \<and> context_invariant t \<sigma> \<gamma> \<theta> \<tau>"
+      using `w = worldline t \<sigma> \<theta> \<tau>` by auto
+  qed
+qed
+
+lemma worldline2_constructible':
+  fixes w :: "'signal worldline2"
+  fixes t :: nat                                     
+  shows "\<exists>\<sigma> \<gamma> \<theta> \<tau>. w = worldline2 t \<sigma> \<theta> \<tau> \<and> context_invariant t \<sigma> \<gamma> \<theta> \<tau>"
+  by (meson destruct_worldline_def worldline2_constructible)
+
+lemma state_worldline2:
+  assumes "context_invariant t \<sigma> \<gamma> \<theta> \<tau>"
+  shows "(\<lambda>s. Rep_worldline (worldline2 t \<sigma> \<theta> \<tau>) s t) = \<sigma>"
+  using assms
+proof (intro ext, transfer')
+  fix s t \<sigma>
+  fix \<gamma> :: "'a event" 
+  fix \<theta> \<tau>
+  assume ci: "context_invariant t \<sigma> \<gamma> \<theta> \<tau>"
+  hence "\<And>n. n < t \<Longrightarrow> lookup \<tau> n = 0"
+    unfolding context_invariant_def by auto
+  have "lookup \<tau> t s = 0 \<or> lookup \<tau> t s \<noteq> 0" by auto
+  moreover
+  { assume "lookup \<tau> t s \<noteq> 0"
+    hence "s \<in> dom (lookup \<tau> t)"      
+      by (metis domIff zero_fun_def zero_map)
+    hence "\<sigma> s = the (lookup \<tau> t s)"
+      using ci unfolding context_invariant_def by auto
+    hence lookup: "lookup \<tau> t s = Some (\<sigma> s)"
+      by (simp add: \<open>s \<in> dom (get_trans \<tau> t)\<close> domD)
+    hence " signal_of2 (\<sigma> s) \<tau> s t = \<sigma> s"
+      using lookup_some_signal_of2'[of "\<tau>" "t" "s" "\<sigma>", OF lookup] by auto
+    hence "worldline t \<sigma> \<theta> \<tau> s t = \<sigma> s"
+      unfolding worldline_def by auto }
+  moreover
+  { assume "lookup \<tau> t s = 0"
+    have "\<forall>k\<in>dom (lookup (to_transaction2 \<tau> s)). t < k"
+    proof (rule ccontr)
+      assume "\<not> (\<forall>k\<in>dom (lookup (to_transaction2 \<tau> s)). t < k)"
+      then obtain k where k_dom: "k \<in> dom (lookup (to_transaction2 \<tau> s))" and "k \<le> t"
+        using leI by blast
+      have "lookup \<tau> k s = 0"
+        using `\<And>n. n < t \<Longrightarrow> lookup \<tau> n = 0` `lookup \<tau> t s = 0` `k \<le> t`
+        by (metis antisym_conv1 zero_fun_def)
+      moreover have "lookup \<tau> k s \<noteq> 0"
+        using k_dom unfolding domIff zero_option_def apply transfer' unfolding to_trans_raw2_def 
+        by auto
+      ultimately show "False"
+        by auto
+    qed
+    hence "inf_time (to_transaction2 \<tau>) s t = None"
+      by (intro inf_time_noneI)
+    hence "signal_of2 (\<sigma> s) \<tau> s t = \<sigma> s"
+      unfolding to_signal2_def comp_def by auto 
+    hence "worldline t \<sigma> \<theta> \<tau> s t = \<sigma> s"
+      unfolding worldline_def by auto }
+  ultimately show "worldline t \<sigma> \<theta> \<tau> s t = \<sigma> s"
+    by auto
+qed
+
+lemma history_worldline2:
+  assumes "context_invariant t \<sigma> \<gamma> \<theta> \<tau>"
+  shows "signal_of2 False (poly_mapping_of_fun (\<lambda>ta. Some \<circ> (\<lambda>s. Rep_worldline (worldline2 t \<sigma> \<theta> \<tau>) s ta)) 0 t) s (t - 1) = 
+         signal_of2 False \<theta> s (t - 1)"
+  using assms
+proof transfer'
+  fix t \<sigma> 
+  fix \<gamma> :: "'a event" 
+  fix \<theta> \<tau> s
+  assume "context_invariant t \<sigma> \<gamma> \<theta> \<tau>"
+  hence "lookup \<theta> t = 0"
+    unfolding context_invariant_def by auto
+  have "0 < t \<or> t = 0" by auto
+  moreover
+  { assume "0 < t"
+    hence "t - 1 < t"
+      by auto
+    have *: "\<And>n.        n \<le> t - 1 \<Longrightarrow>
+         lookup (poly_mapping_of_fun (\<lambda>taa. Some \<circ> (\<lambda>s. worldline t \<sigma> \<theta> \<tau> s taa)) 0 t) n =
+         lookup (poly_mapping_of_fun (\<lambda>taa. Some \<circ> (\<lambda>s. signal_of2 False \<theta> s taa)) 0 t) n"
+      apply transfer' unfolding worldline_def by auto
+    have " signal_of2 False (poly_mapping_of_fun (\<lambda>ta. Some \<circ> (\<lambda>s. worldline t \<sigma> \<theta> \<tau> s ta)) 0 t) s (t - 1) = 
+           signal_of2 False (poly_mapping_of_fun (\<lambda>taa. Some \<circ> (\<lambda>s. signal_of2 False \<theta> s taa)) 0 t) s (t - 1)"
+      using signal_of2_lookup_same[OF *] by auto
+    also have "... = signal_of2 False \<theta> s (t - 1)"
+      using signal_of2_poly_mapping_fun[OF `t - 1 < t`] by metis
+    finally have "signal_of2 False (poly_mapping_of_fun (\<lambda>ta. Some \<circ> (\<lambda>s. worldline t \<sigma> \<theta> \<tau> s ta)) 0 t) s (t - 1) = signal_of2 False \<theta> s (t - 1)"
+      by auto }
+  moreover
+  { assume "t = 0"
+    hence "signal_of2 False (poly_mapping_of_fun (\<lambda>ta. Some \<circ> (\<lambda>s. worldline t \<sigma> \<theta> \<tau> s ta)) 0 t) s (t - 1) = 
+           signal_of2 False (poly_mapping_of_fun (\<lambda>ta. Some \<circ> (\<lambda>s. worldline 0 \<sigma> \<theta> \<tau> s ta)) 0 0) s 0"
+      by auto
+    also have "... =  signal_of2 False 0 s 0"
+      unfolding poly_mapping_of_fun_empty_set  by auto
+    also have "... = signal_of2 False \<theta> s 0"
+      using `lookup \<theta> t = 0` unfolding `t = 0` using signal_of2_zero 
+      by (metis signal_of2_empty zero_fun_def)
+    also have "... = signal_of2 False \<theta> s (t - 1)"
+      using `t = 0` by auto
+    finally have "signal_of2 False (poly_mapping_of_fun (\<lambda>ta. Some \<circ> (\<lambda>s. worldline t \<sigma> \<theta> \<tau> s ta)) 0 t) s (t - 1) = signal_of2 False \<theta> s (t - 1)"
+      by auto }
+  ultimately show "signal_of2 False (poly_mapping_of_fun (\<lambda>ta. Some \<circ> (\<lambda>s. worldline t \<sigma> \<theta> \<tau> s ta)) 0 t) s (t - 1) = signal_of2 False \<theta> s (t - 1)"
+    by auto 
+qed
+
+lemma beh_of_worldline:
+  assumes "context_invariant t \<sigma> \<gamma> \<theta> \<tau>"
+  shows "\<And>k. signal_of2 False (poly_mapping_of_fun (\<lambda>ta. Some \<circ> (\<lambda>s. Rep_worldline (worldline2 t \<sigma> \<theta> \<tau>) s ta)) 0 t) s k = 
+             signal_of2 False \<theta> s k"
+  using assms
+proof transfer'
+  fix k t \<sigma> 
+  fix \<gamma> :: "'a event" 
+  fix \<theta> \<tau> s 
+  assume "context_invariant t \<sigma> \<gamma> \<theta> \<tau>"
+  hence "lookup \<theta> t = 0"
+    unfolding context_invariant_def by auto
+  have *: "\<And>n.       
+       lookup (poly_mapping_of_fun (\<lambda>taa. Some \<circ> (\<lambda>s. worldline t \<sigma> \<theta> \<tau> s taa)) 0 t) n =
+       lookup (poly_mapping_of_fun (\<lambda>taa. Some \<circ> (\<lambda>s. signal_of2 False \<theta> s taa)) 0 t) n"
+    apply transfer' unfolding worldline_def by auto
+  have **: " signal_of2 False (poly_mapping_of_fun (\<lambda>ta. Some \<circ> (\<lambda>s. worldline t \<sigma> \<theta> \<tau> s ta)) 0 t) s k = 
+         signal_of2 False (poly_mapping_of_fun (\<lambda>taa. Some \<circ> (\<lambda>s. signal_of2 False \<theta> s taa)) 0 t) s k"
+    using signal_of2_lookup_same[OF *] by auto
+  have "k < t \<or> t \<le> k"
+    by auto
+  moreover 
+  { assume "k < t"
+    have "signal_of2 False (poly_mapping_of_fun (\<lambda>taa. Some \<circ> (\<lambda>s. signal_of2 False \<theta> s taa)) 0 t) s k 
+          = signal_of2 False \<theta> s (k)"
+      using signal_of2_poly_mapping_fun[OF `k < t`] by metis
+    hence "signal_of2 False (poly_mapping_of_fun (\<lambda>ta. Some \<circ> (\<lambda>s. worldline t \<sigma> \<theta> \<tau> s ta)) 0 t) s k = signal_of2 False \<theta> s k"
+      using ** by auto }
+  moreover
+  { assume "t \<le> k"
+    have "0 < t \<or> t = 0"
+      by auto
+    moreover
+    { assume "0 < t"
+      hence "t - 1 < k" and "t - 1 < t"
+        using `0 < t` `t \<le> k` by auto
+      have history: "\<And>n. t - 1 < n \<Longrightarrow> n \<le> k \<Longrightarrow> lookup \<theta> n = 0"
+        using `context_invariant t \<sigma> \<gamma> \<theta> \<tau>` unfolding context_invariant_def by auto
+      have "\<And>n. t - 1 < n \<Longrightarrow> n \<le> k \<Longrightarrow> lookup (poly_mapping_of_fun (\<lambda>taa. Some \<circ> (\<lambda>s. signal_of2 False \<theta> s taa)) 0 t) n = 0"
+        apply transfer' by auto
+      with signal_of2_less_ind[OF this]
+      have "signal_of2 False (poly_mapping_of_fun (\<lambda>taa. Some \<circ> (\<lambda>s. signal_of2 False \<theta> s taa)) 0 t) s k = 
+             signal_of2 False (poly_mapping_of_fun (\<lambda>taa. Some \<circ> (\<lambda>s. signal_of2 False \<theta> s taa)) 0 t) s (t - 1)"
+        using `t - 1 < k` by auto
+      also have "... = signal_of2 False \<theta> s (t - 1)"
+        using signal_of2_poly_mapping_fun[OF `t -1 < t`, where w="signal_of2 False \<theta>"] by auto
+      also have "... = signal_of2 False \<theta> s k"
+        using signal_of2_less_ind[OF history] `t - 1 < k` by auto
+      finally have "signal_of2 False (poly_mapping_of_fun (\<lambda>ta. Some \<circ> (\<lambda>s. worldline t \<sigma> \<theta> \<tau> s ta)) 0 t) s k = signal_of2 False \<theta> s k"
+        using ** by auto }
+    moreover
+    { assume "t = 0"
+      hence "signal_of2 False (poly_mapping_of_fun (\<lambda>taa. Some \<circ> (\<lambda>s. signal_of2 False \<theta> s taa)) 0 t) s k = 
+            signal_of2 False (poly_mapping_of_fun (\<lambda>taa. Some \<circ> (\<lambda>s. signal_of2 False \<theta> s taa)) 0 0) s k"
+        by auto
+      also have "... = signal_of2 False 0 s k"
+        unfolding poly_mapping_of_fun_empty_set by auto
+      also have "... = False"
+        using signal_of2_empty by fastforce
+      finally have step: "signal_of2 False (poly_mapping_of_fun (\<lambda>taa. Some \<circ> (\<lambda>s. signal_of2 False \<theta> s taa)) 0 t) s k = False"
+        using ** by auto
+      have history: "\<And>n. t - 1 < n \<Longrightarrow> n \<le> k \<Longrightarrow> lookup \<theta> n = 0"
+        using `context_invariant t \<sigma> \<gamma> \<theta> \<tau>` unfolding context_invariant_def by auto
+      hence "signal_of2 False \<theta> s k = signal_of2 False \<theta> s 0"
+        using signal_of2_less_ind[OF history] `t \<le> k` unfolding `t = 0` by force
+      also have "... = False"
+        using `lookup \<theta> t = 0`  by (metis \<open>t = 0\<close> signal_of2_zero zero_fun_def)
+      finally have "signal_of2 False \<theta> s k = False"
+        by auto
+      hence "signal_of2 False (poly_mapping_of_fun (\<lambda>ta. Some \<circ> (\<lambda>s. worldline t \<sigma> \<theta> \<tau> s ta)) 0 t) s k = signal_of2 False \<theta> s k"
+        using step using "**" by blast }
+    ultimately have "signal_of2 False (poly_mapping_of_fun (\<lambda>ta. Some \<circ> (\<lambda>s. worldline t \<sigma> \<theta> \<tau> s ta)) 0 t) s k = signal_of2 False \<theta> s k"
+      by auto }
+  ultimately show "signal_of2 False (poly_mapping_of_fun (\<lambda>ta. Some \<circ> (\<lambda>s. worldline t \<sigma> \<theta> \<tau> s ta)) 0 t) s k = signal_of2 False \<theta> s k"
+    by auto
+qed
+
+lemma event_worldline2:
+  assumes "context_invariant t \<sigma> \<gamma> \<theta> \<tau>"
+  shows "{s. Rep_worldline (worldline2 t \<sigma> \<theta> \<tau>) s t \<noteq> signal_of2 False (poly_mapping_of_fun (\<lambda>ta. Some \<circ> (\<lambda>s. Rep_worldline (worldline2 t \<sigma> \<theta> \<tau>) s ta)) 0 t) s (t - 1)} = \<gamma>"
+  using assms state_worldline2[OF assms]
+proof transfer'
+  fix t \<sigma> 
+  fix \<gamma> :: "'a event" 
+  fix \<theta> \<tau>
+  assume "context_invariant t \<sigma> \<gamma> \<theta> \<tau>"
+  assume *: "(\<lambda>s. worldline t \<sigma> \<theta> \<tau> s t) = \<sigma>"
+  have **: "\<gamma> = {s. \<sigma> s \<noteq> signal_of2 False \<theta> s (t - 1)}"  
+    using `context_invariant t \<sigma> \<gamma> \<theta> \<tau>` unfolding context_invariant_def by auto
+  have "{s. worldline t \<sigma> \<theta> \<tau> s t \<noteq> signal_of2 False (poly_mapping_of_fun (\<lambda>ta. Some \<circ> (\<lambda>s. worldline t \<sigma> \<theta> \<tau> s ta)) 0 t) s (t - 1)} = 
+        {s. \<sigma> s \<noteq> signal_of2 False (poly_mapping_of_fun (\<lambda>ta. Some \<circ> (\<lambda>s. worldline t \<sigma> \<theta> \<tau> s ta)) 0 t) s (t - 1)}"
+    using * by metis
+  moreover have "\<And>s. signal_of2 False \<theta> s (t - 1) = 
+            signal_of2 False (poly_mapping_of_fun (\<lambda>ta. Some \<circ> (\<lambda>s. worldline t \<sigma> \<theta> \<tau> s ta)) 0 t) s (t - 1)" 
+    using history_worldline2 by (metis \<open>context_invariant t \<sigma> \<gamma> \<theta> \<tau>\<close> worldline2.rep_eq)
+  ultimately have "{s. worldline t \<sigma> \<theta> \<tau> s t \<noteq> signal_of2 False (poly_mapping_of_fun (\<lambda>ta. Some \<circ> (\<lambda>s. worldline t \<sigma> \<theta> \<tau> s ta)) 0 t) s (t - 1)} =
+                   {s. \<sigma> s \<noteq> signal_of2 False \<theta> s (t - 1)}"
+    by auto
+  thus " {s. worldline t \<sigma> \<theta> \<tau> s t \<noteq> signal_of2 False (poly_mapping_of_fun (\<lambda>ta. Some \<circ> (\<lambda>s. worldline t \<sigma> \<theta> \<tau> s ta)) 0 t) s (t - 1)} = \<gamma>"
+    using ** by auto
+qed
+
+lemma transaction_worldline2:
+  assumes "context_invariant t \<sigma> \<gamma> \<theta> \<tau>"
+  shows "\<And>k s . signal_of2 (\<sigma> s) (derivative_raw (Rep_worldline (worldline2 t \<sigma> \<theta> \<tau>)) (worldline_deg (worldline2 t \<sigma> \<theta> \<tau>)) t) s k = 
+                signal_of2 (\<sigma> s) \<tau> s k"
+  using assms unfolding worldline_deg_def
+proof transfer'
+  fix k s t \<sigma>
+  fix \<gamma> :: "'a event"
+  fix \<theta> \<tau>
+  assume "context_invariant t \<sigma> \<gamma> \<theta> \<tau>"
+  define deg where "deg = (LEAST n. \<forall>ta>n. \<forall>s. worldline t \<sigma> \<theta> \<tau> s ta = worldline t \<sigma> \<theta> \<tau> s n)"
+  have deg_prop: "\<forall>ta > deg. \<forall>s. worldline t \<sigma> \<theta> \<tau> s ta = worldline t \<sigma> \<theta> \<tau> s deg"
+    using LeastI_ex[OF exists_quiesce_worldline[OF `context_invariant t \<sigma> \<gamma> \<theta> \<tau>`]] unfolding deg_def
+    by blast
+  have "k < t \<or> t \<le> k \<and> k \<le> deg \<or> deg < k"
+    by auto
+  moreover
+  { assume "k < t"
+    have "signal_of2 (\<sigma> s) (derivative_raw (worldline t \<sigma> \<theta> \<tau>) deg t) s k = \<sigma> s"
+      using signal_of2_derivative_before_now \<open>k < t\<close> by fastforce  
+    moreover have "signal_of2 (\<sigma> s) \<tau> s k = \<sigma> s"
+    proof -
+      have "\<forall>n\<in>dom (lookup (to_transaction2 \<tau> s)). k < n"
+      proof (rule ccontr)
+        assume "\<not> (\<forall>n\<in>dom (lookup (to_transaction2 \<tau> s)). k < n)"
+        then obtain n where "n \<in> dom (lookup (to_transaction2 \<tau> s))" and "n \<le> k"
+          using leI by blast
+        hence "lookup \<tau> n = 0"
+          using `context_invariant t \<sigma> \<gamma> \<theta> \<tau>` unfolding context_invariant_def using `k < t`
+          by auto
+        hence "n \<notin> dom (lookup (to_transaction2 \<tau> s))"
+          apply transfer' unfolding to_trans_raw2_def  by (simp add: domIff zero_map)
+        with `n \<in> dom (lookup (to_transaction2 \<tau> s))` show False by auto
+      qed
+      hence "inf_time (to_transaction2 \<tau>) s k = None"
+        by (rule inf_time_noneI)
+      thus ?thesis
+        unfolding to_signal2_def comp_def by auto
+    qed
+    ultimately have "signal_of2 (\<sigma> s) (derivative_raw (worldline t \<sigma> \<theta> \<tau>) deg t) s k = 
+                     signal_of2 (\<sigma> s) \<tau> s k" 
+      by auto }
+  moreover
+  { assume "t \<le> k \<and> k \<le> deg"
+    hence "signal_of2 (\<sigma> s) (derivative_raw (worldline t \<sigma> \<theta> \<tau>) deg t) s k = (worldline t \<sigma> \<theta> \<tau>) s k"
+      using signal_of2_derivative_raw by metis
+    also have "... = signal_of2 (\<sigma> s) \<tau> s k"
+      unfolding worldline_def using `t \<le> k \<and> k \<le> deg` by auto
+    finally have "signal_of2 (\<sigma> s) (derivative_raw (worldline t \<sigma> \<theta> \<tau>) deg t) s k = 
+                     signal_of2 (\<sigma> s) \<tau> s k"
+      by auto }
+  moreover
+  { assume "deg < k"
+    have "t \<le> deg \<or> deg < t" by auto
+    moreover
+    { assume "t \<le> deg"
+      hence "signal_of2 (\<sigma> s) (derivative_raw (worldline t \<sigma> \<theta> \<tau>) deg t) s k = (worldline t \<sigma> \<theta> \<tau>) s deg"
+        using signal_of2_derivative_raw2[OF _ `deg < k`] by metis
+      also have "... =  signal_of2 (\<sigma> s) \<tau> s deg"
+        unfolding worldline_def using `t \<le> deg` by auto
+      also have "... = signal_of2 (\<sigma> s) \<tau> s k"
+        using deg_prop `deg < k` `t \<le> deg` unfolding worldline_def by auto
+      finally have "signal_of2 (\<sigma> s) (derivative_raw (worldline t \<sigma> \<theta> \<tau>) deg t) s k = 
+                    signal_of2 (\<sigma> s) \<tau> s k"
+        by auto }
+    moreover
+    { assume "deg < t"
+      hence "derivative_raw (worldline t \<sigma> \<theta> \<tau>) deg t = 0"
+        using derivative_raw_zero by auto
+      hence "signal_of2 (\<sigma> s) (derivative_raw (worldline t \<sigma> \<theta> \<tau>) deg t) s k = \<sigma> s"
+        using signal_of2_derivative_raw_degree_lt_now[OF `deg < t`] by metis
+      also have "... = signal_of2 (\<sigma> s) \<tau> s k"
+      proof -
+        have "worldline t \<sigma> \<theta> \<tau> s k = worldline t \<sigma> \<theta> \<tau> s t"
+          using deg_prop `k > deg` `t > deg` by auto
+        have "k < t \<or> t \<le> k" by auto
+        moreover
+        { assume "k < t"
+          have "\<forall>n\<in>dom (lookup (to_transaction2 \<tau> s)). k < n"
+          proof (rule ccontr)
+            assume "\<not> (\<forall>n\<in>dom (lookup (to_transaction2 \<tau> s)). k < n)"
+            then obtain n where "n \<in> dom (lookup (to_transaction2 \<tau> s))" and "n \<le> k"
+              using leI by blast
+            hence "lookup \<tau> n = 0"
+              using `context_invariant t \<sigma> \<gamma> \<theta> \<tau>` unfolding context_invariant_def using `k < t`
+              by auto
+            hence "n \<notin> dom (lookup (to_transaction2 \<tau> s))"
+              apply transfer' unfolding to_trans_raw2_def  by (simp add: domIff zero_map)
+            thus False
+              by (simp add: \<open>n \<in> dom (lookup (to_transaction2 \<tau> s))\<close>)
+          qed
+          hence "inf_time (to_transaction2 \<tau>) s k  = None"
+            by (rule inf_time_noneI)
+          hence ?thesis
+            unfolding to_signal2_def comp_def by auto }
+        moreover
+        { assume "t \<le> k"
+          hence "worldline t \<sigma> \<theta> \<tau> s k = signal_of2 (\<sigma> s) \<tau> s k"
+            unfolding worldline_def by auto
+          have "worldline t \<sigma> \<theta> \<tau> s t = signal_of2 (\<sigma> s) \<tau> s t"
+            unfolding worldline_def by auto
+          also have "... = \<sigma> s"
+            using `context_invariant t \<sigma> \<gamma> \<theta> \<tau>` 
+            by (metis calculation state_worldline2 worldline2.rep_eq)
+          finally have "worldline t \<sigma> \<theta> \<tau> s t = \<sigma> s"
+            by auto
+          hence ?thesis
+            using \<open>worldline t \<sigma> \<theta> \<tau> s k = signal_of2 (\<sigma> s) \<tau> s k\<close> 
+            \<open>worldline t \<sigma> \<theta> \<tau> s k = worldline t \<sigma> \<theta> \<tau> s t\<close> by blast }
+        ultimately show ?thesis by auto 
+      qed
+      finally have "signal_of2 (\<sigma> s) (derivative_raw (worldline t \<sigma> \<theta> \<tau>) deg t) s k = 
+                    signal_of2 (\<sigma> s) \<tau> s k"
+        by auto }
+    ultimately have "signal_of2 (\<sigma> s) (derivative_raw (worldline t \<sigma> \<theta> \<tau>) deg t) s k = 
+                    signal_of2 (\<sigma> s) \<tau> s k" by auto }
+  ultimately have "signal_of2 (\<sigma> s) (derivative_raw (worldline t \<sigma> \<theta> \<tau>) deg t) s k = 
+                    signal_of2 (\<sigma> s) \<tau> s k" by auto
+  thus "signal_of2 (\<sigma> s) (derivative_raw (worldline t \<sigma> \<theta> \<tau>) (LEAST n. \<forall>ta>n. \<forall>s. worldline t \<sigma> \<theta> \<tau> s ta = worldline t \<sigma> \<theta> \<tau> s n) t) s k = 
+        signal_of2 (\<sigma> s) \<tau> s k"
+    unfolding deg_def by auto
+qed
+
+lemma destruct_worldline_correctness:               
+  assumes "context_invariant t \<sigma> \<gamma> \<theta> \<tau>"
+  assumes "destruct_worldline (worldline2 t \<sigma> \<theta> \<tau>) t = (\<sigma>', \<gamma>', \<theta>', \<tau>')"
+  shows "\<sigma> = \<sigma>'" and "\<gamma> = \<gamma>'" 
+    and "\<And>k s. signal_of2 False \<theta> s k = signal_of2 False \<theta>' s k"
+    and "\<And>k s. signal_of2 (\<sigma> s) \<tau> s k = signal_of2 (\<sigma> s) \<tau>' s k"
+  using assms(2) state_worldline2[OF assms(1)] event_worldline2[OF assms(1)] beh_of_worldline[OF assms(1)]
+  transaction_worldline2[OF assms(1)] unfolding destruct_worldline_def Let_def by auto
+
+text \<open>Ideally, we want the destructor @{term "destruct_worldline"} is the inverse of the constructor
+@{term "worldline2"}. Unfortunately this is not the case here. Note that in the lemma above, 
+the states are the same @{term "\<sigma> = \<sigma>'"}, the events are the same @{term "\<gamma> = \<gamma>'"} but not with 
+the history (or behaviours) @{term "\<theta>"} @{term "\<theta>'"} and the transactions @{term "\<tau>"} @{term "\<tau>'"}. 
+Why is this the case? 
+
+To answer this question, we need to explain the ``inverse'' function of the derivative, i.e., 
+``integral'' which is achieved via the function @{term "signal_of2"}. It is basically the function 
+to turn a transaction into a signal. This ``integral'' function runs through over time, note if 
+there is a mapping, and change the signal value according to this mapping. It is basically like 
+integration function in real calculus, but the value can only either be ``0'' or ``1''. 
+
+The reason why we cannot have the equality @{term "\<tau> = \<tau>'"} and @{term "\<theta> = \<theta>'"} is because a
+worldline does not have a unique ``derivative''. Suppose that the transaction @{term "\<tau>"} maps the
+signal @{term "sig\<^sub>1 :: 'signal"} to @{term "True :: val"} at time 0 and none at other times.
+Suppose also that we have another transaction @{term "\<tau>'"} which is the same with @{term "\<tau>"} except
+that it also maps @{term "sig\<^sub>1 :: 'signal"} to @{term "True :: val"} at time 1. When we
+``integrate'' both of these transactions, we will obtain an identical worldline; posting (setting) a
+signal to @{term "True"} where we have previously posted (maps) the same value is futile.
+
+However, even though the transaction @{term "\<tau>'"} and history @{term "\<theta>"} are not guaranteed to be 
+the same with @{term "\<tau>"} and @{term "\<theta>"} any longer, the ``integrals'' are still the same; see
+property 3 and 4 in the theorem above.\<close>
+
+definition world_seq_exec :: "'signal worldline2 \<Rightarrow> nat \<Rightarrow> 'signal seq_stmt \<Rightarrow> 'signal worldline2" where 
+  "world_seq_exec w t s = (let (\<sigma>, \<gamma>, \<theta>, \<tau>) = destruct_worldline w t; 
+                                         \<tau>' = b_seq_exec t \<sigma> \<gamma> \<theta> s \<tau> 
+                           in worldline2 t \<sigma> \<theta> \<tau>')"
+
+abbreviation world_seq_exec_abb :: "'signal worldline2 \<Rightarrow> nat \<Rightarrow> 'signal seq_stmt \<Rightarrow> 'signal worldline2 \<Rightarrow> bool" 
+  ("(_, _ , _) \<Rightarrow>\<^sub>s _")
+  where "world_seq_exec_abb w t s w' \<equiv> (world_seq_exec w t s = w')"
+
+(* Diagram for lifting the sequential execution to the worldline level
+ *
+ *         w, t                    \<Rightarrow>\<^sub>s          w', t
+ *           \<down>                                  \<up>
+ *   destruct_worldline                      worldline2 t \<sigma> \<theta> \<tau>'
+ *           \<down>                                  \<up>
+ *         t, \<sigma>, \<gamma>, \<theta> \<turnstile> <s, \<tau>>    \<longrightarrow>\<^sub>s          \<tau>'
+ *
+ *)
+
+definition
+seq_hoare_valid2 :: "nat \<Rightarrow> 'signal assn2 \<Rightarrow> 'signal seq_stmt \<Rightarrow> 'signal assn2 \<Rightarrow> bool" ("\<Turnstile>\<^sub>_ [(1_)]/ (_)/ [(1_)]" 50)
+where "\<Turnstile>\<^sub>t [P] s [Q] \<longleftrightarrow>  (\<forall>w w'.  P w \<and> (w, t, s \<Rightarrow>\<^sub>s w') \<longrightarrow> Q w')"
+
+text \<open>This is a cleaner definition of the validity compared to @{term "seq_hoare_valid"} in 
+@{theory "Draft.VHDL_Hoare"}. This also has the same spirit as the definition of validity in 
+@{theory_text "Hoare"}.\<close>
+
+lemma beval_cong:
+  assumes "\<And>k s. signal_of2 False \<theta>1 s k = signal_of2 False \<theta>2 s k"
+  shows "beval t \<sigma> \<gamma> \<theta>1 g \<longleftrightarrow> beval t \<sigma> \<gamma> \<theta>2 g"
+  using assms by (induction g, auto)
+
+lemma signal_of2_eq_is_stable:
+  assumes "is_stable dly \<tau>1 t sig (\<sigma> sig)"
+  assumes "\<And>k s. signal_of2 (\<sigma> s) \<tau>1 s k = signal_of2 (\<sigma> s) \<tau>2 s k"
+  assumes "\<And>n. n < t \<Longrightarrow> lookup \<tau>1 n = 0"
+  assumes "\<And>s. s \<in> dom (lookup \<tau>1 t) \<Longrightarrow> \<sigma> s = the (lookup \<tau>1 t s)"
+  shows "is_stable dly \<tau>2 t sig (\<sigma> sig)"
+  unfolding is_stable_correct 
+proof safe
+  fix m
+  assume "t < m"
+  assume "m \<le> t + dly"
+  obtain x where "lookup \<tau>2 m sig = None \<or> lookup \<tau>2 m sig = Some x"
+    by (meson not_None_eq)
+  moreover
+  { assume "lookup \<tau>2 m sig = None"
+    hence "check (get_trans \<tau>2 m) sig (\<sigma> sig)" by auto }
+  moreover
+  { assume "lookup \<tau>2 m sig = Some x"
+    hence "signal_of2 (\<sigma> sig) \<tau>2 sig m = x"
+      using lookup_some_signal_of2' by fastforce 
+    hence "signal_of2 (\<sigma> sig) \<tau>1 sig m = x"
+      using assms(2) by auto
+    have *: "lookup \<tau>1 m sig = None \<or> lookup \<tau>1 m sig = Some x"
+    proof (rule ccontr)
+      assume "\<not> (lookup \<tau>1 m sig = None \<or> lookup \<tau>1 m sig = Some x)"
+      hence "lookup \<tau>1 m sig \<noteq> None \<and> lookup \<tau>1 m sig \<noteq> Some x"
+        by auto
+      then obtain y where "y \<noteq> x" and "lookup \<tau>1 m sig = Some y"
+        using domD domIff by auto
+      hence "signal_of2 (\<sigma> sig) \<tau>1 sig m = y"
+        using lookup_some_signal_of2' by fastforce
+      with `signal_of2 (\<sigma> sig) \<tau>1 sig m = x` and `y \<noteq> x` show False
+        by auto
+    qed
+    moreover
+    { assume "lookup \<tau>1 m sig = Some x"
+      hence "x = \<sigma> sig"
+        using assms(1) unfolding is_stable_correct using `t < m` `m \<le> t + dly`  by auto
+      hence "check (lookup \<tau>2 m) sig (\<sigma> sig)"
+        using `lookup \<tau>2 m sig = Some x` by auto }
+    moreover
+    { assume "lookup \<tau>1 m sig = None"
+      obtain k where "find (\<lambda>x. lookup \<tau>1 x sig \<noteq> None) (rev [0..< m]) = None \<or>
+                      find (\<lambda>x. lookup \<tau>1 x sig \<noteq> None) (rev [0..< m]) = Some k"
+        using option.exhaust_sel by blast
+      moreover
+      { assume "find (\<lambda>x. lookup \<tau>1 x sig \<noteq> None) (rev [0..< m]) = None"
+        hence "\<not> (\<exists>x. x \<in> set [0 ..< m] \<and> lookup \<tau>1 x sig \<noteq> None)"
+          unfolding find_None_iff by auto
+        hence "\<And>x. x < m \<Longrightarrow> lookup \<tau>1 x sig = None"
+          by auto
+        hence **: "\<And>x. x \<le> m \<Longrightarrow> lookup \<tau>1 x sig = None"
+          using `lookup \<tau>1 m sig = None` using nat_less_le by blast
+        have "signal_of2 (\<sigma> sig) \<tau>1 sig m = \<sigma> sig"
+        proof -
+          have "\<forall>t\<in>dom (lookup (to_transaction2 \<tau>1 sig)). m < t"
+          proof (rule ccontr)
+            assume "\<not>(\<forall>t\<in>dom (lookup (to_transaction2 \<tau>1 sig)). m < t)"
+            then obtain t where "t \<in>dom (lookup (to_transaction2 \<tau>1 sig))" and "t \<le> m"
+              using leI by blast
+            with ** have "lookup \<tau>1 t sig = None"
+              by auto
+            hence "t \<notin> dom (lookup (to_transaction2 \<tau>1 sig))"
+              apply transfer' unfolding to_trans_raw2_def by auto
+            thus False
+              using \<open>t \<in> dom (lookup (to_transaction2 \<tau>1 sig))\<close> by blast
+          qed
+          hence " inf_time (to_transaction2 \<tau>1) sig m = None"
+            by (rule inf_time_noneI)
+          thus ?thesis
+            unfolding to_signal2_def comp_def by auto
+        qed
+        hence "x = \<sigma> sig"
+          using `signal_of2 (\<sigma> sig) \<tau>1 sig m = x` by auto
+        hence "check (lookup \<tau>2 m) sig (\<sigma> sig)"
+          using `lookup \<tau>2 m sig = Some x` by auto }
+      moreover
+      { assume "find (\<lambda>x. lookup \<tau>1 x sig \<noteq> None) (rev [0..< m]) = Some k"
+        hence " \<exists>i<length (rev [0..<m]). get_trans \<tau>1 (rev [0..<m] ! i) sig \<noteq> None 
+                                       \<and> k = rev [0..<m] ! i 
+                                       \<and> (\<forall>j<i. \<not> get_trans \<tau>1 (rev [0..<m] ! j) sig \<noteq> None)"
+          unfolding find_Some_iff by auto
+        then obtain i where "i<length (rev [0..<m])" and "get_trans \<tau>1 (rev [0..<m] ! i) sig \<noteq> None"
+                      and "k = rev [0..<m] ! i " and quant: "\<forall>j<i.  lookup \<tau>1 (rev [0..<m] ! j) sig = None"
+          by auto
+        have "k = m - i - 1" using `k = rev [0..<m] ! i` 
+          by (metis One_nat_def \<open>i < length (rev [0..<m])\<close> add.left_neutral add.right_neutral 
+              add_Suc_right diff_diff_add diff_less diff_zero length_rev length_upt nat_less_le 
+              neq0_conv nth_upt rev_nth zero_less_Suc zero_order(2))
+        hence iless: "i < length ([0..<m])"
+          using `i<length (rev [0..<m])` by auto
+        have "lookup \<tau>1 k sig \<noteq> None" 
+          using rev_nth[OF iless] `lookup \<tau>1 (rev [0..<m] ! i) sig \<noteq> None` `k = m - i - 1`
+          using \<open>k = rev [0..<m] ! i\<close> by auto          
+        have "\<And>j. j > k \<Longrightarrow>  j < m \<Longrightarrow> lookup \<tau>1 j sig = None"
+        proof -
+          fix j
+          assume "k < j" and "j < m"
+          define j' where "j' = m - j - 1"
+          have "m - i - 1 < j"
+            using `k < j` unfolding `k  = m - i - 1` by auto
+          hence "j' < i"
+            unfolding j'_def  using `j < m` by linarith
+          hence lookup: "lookup \<tau>1 (rev [0..< m] ! j') sig = None"
+            using quant by auto
+          have "j' < m"
+            unfolding j'_def using `j < m` by auto
+          with rev_nth have "rev [0 ..< m] ! j' = [0 ..< m] ! j"
+            unfolding j'_def  by (simp add: rev_nth Suc_diff_Suc \<open>j < m\<close> less_imp_le_nat)
+          with lookup have "get_trans \<tau>1 ([0 ..< m] ! j) sig = None"
+            by auto
+          thus "get_trans \<tau>1 j sig = None"
+            using nth_upt `j < m` by auto
+        qed
+        hence ind: "\<And>j. k < j \<Longrightarrow> j \<le> m \<Longrightarrow> lookup \<tau>1 j sig = 0"
+          using `lookup \<tau>1 m sig = None` using dual_order.order_iff_strict  zero_option_def by fastforce
+        have "t \<le> k" 
+        proof (rule ccontr)
+          assume "\<not> (t \<le> k)" hence "k < t" by auto
+          hence "lookup \<tau>1 k sig = None"
+            using assms(3)  by (simp add: zero_map)
+          with `lookup \<tau>1 k sig \<noteq> None` show "False" by auto
+        qed
+        have "k < m"
+          using \<open>i < length (rev [0..<m])\<close> \<open>k = m - i - 1\<close> by auto
+        have "signal_of2 (\<sigma> sig) \<tau>1 sig m = signal_of2 (\<sigma> sig) \<tau>1 sig k"
+          using signal_of2_less_ind'[OF ind `k < m`] by auto
+        hence "signal_of2 (\<sigma> sig) \<tau>1 sig k = x"
+          using `signal_of2 (\<sigma> sig) \<tau>1 sig m = x` by auto
+        have "lookup \<tau>1 k sig = None \<or> lookup \<tau>1 k sig = Some x"
+        proof (rule ccontr)
+          assume "\<not> (lookup \<tau>1 k sig = None \<or> lookup \<tau>1 k sig = Some x)"
+          hence "lookup \<tau>1 k sig \<noteq> None \<and> lookup \<tau>1 k sig \<noteq> Some x"
+            by auto
+          then obtain y where "y \<noteq> x" and "lookup \<tau>1 k sig = Some y"
+            using domD domIff by auto
+          hence "signal_of2 (\<sigma> sig) \<tau>1 sig k = y"
+            using lookup_some_signal_of2' by fastforce
+          with `signal_of2 (\<sigma> sig) \<tau>1 sig k = x` and `y \<noteq> x` show False
+            by auto
+        qed
+        with `lookup \<tau>1 k sig \<noteq> None` have "lookup \<tau>1 k sig = Some x"
+          by auto
+        have "t < k \<or> k = t"
+          using `t \<le> k` by auto
+        moreover
+        { assume "t < k"
+          hence "x = \<sigma> sig"
+            using `lookup \<tau>1 k sig = Some x` assms(1) unfolding is_stable_correct 
+            using `t < k` `k < m` `m \<le> t + dly` by auto
+          hence "check (lookup \<tau>2 m) sig (\<sigma> sig)"
+            using `lookup \<tau>2 m sig = Some x` by auto }
+        moreover
+        { assume "t = k"
+          hence "x = \<sigma> sig"
+            using assms(4) `lookup \<tau>1 k sig = Some x`  by (simp add: domIff) 
+          hence "check (lookup \<tau>2 m) sig (\<sigma> sig)"
+            using `lookup \<tau>2 m sig = Some x` by auto }          
+        ultimately have "check (lookup \<tau>2 m) sig (\<sigma> sig)"
+          by auto }
+      ultimately have "check (lookup \<tau>2 m) sig (\<sigma> sig)"
+        by auto }
+    ultimately have "check (lookup \<tau>2 m) sig (\<sigma> sig)"
+      by auto }
+  ultimately show "check (lookup \<tau>2 m) sig (\<sigma> sig)"
+    by auto
+qed
+
+lemma signal_of2_eq_is_stable_eq:
+  assumes "\<And>n. n < t \<Longrightarrow> lookup \<tau>1 n = 0"
+  assumes "\<And>s. s \<in> dom (lookup \<tau>1 t) \<Longrightarrow> \<sigma> s = the (lookup \<tau>1 t s)"
+  assumes "\<And>n. n < t \<Longrightarrow> lookup \<tau>2 n = 0"
+  assumes "\<And>s. s \<in> dom (lookup \<tau>2 t) \<Longrightarrow> \<sigma> s = the (lookup \<tau>2 t s)"
+  assumes "\<And>k s. signal_of2 (\<sigma> s) \<tau>1 s k = signal_of2 (\<sigma> s) \<tau>2 s k"
+  shows "is_stable dly \<tau>1 t sig (\<sigma> sig) \<longleftrightarrow> is_stable dly \<tau>2 t sig (\<sigma> sig)"  
+proof 
+  assume "is_stable dly \<tau>1 t sig (\<sigma> sig)"
+  with signal_of2_eq_is_stable[OF _ assms(5) assms(1-2)] show "is_stable dly \<tau>2 t sig (\<sigma> sig)"
+    by auto
+next
+  assume "is_stable dly \<tau>2 t sig (\<sigma> sig)"
+  with signal_of2_eq_is_stable[OF _ sym[OF assms(5)] assms(3-4)] show "is_stable dly \<tau>1 t sig (\<sigma> sig)"
+    by auto
+qed
+
+lemma signal_of2_purge_not_affected:
+  assumes "s \<noteq> sig"
+  shows "signal_of2 (\<sigma> s) (purge dly \<tau>1 t sig (\<sigma> sig)) s k = signal_of2 (\<sigma> s) \<tau>1 s k"
+proof -
+  have "\<And>n. lookup (to_transaction2 (purge dly \<tau>1 t sig (\<sigma> sig)) s) n = lookup (to_transaction2 \<tau>1 s) n"
+    using assms apply transfer' unfolding to_trans_raw2_def  by (simp add: purge_raw_does_not_affect_other_sig)
+  from signal_of2_lookup_sig_same[OF this] show ?thesis by auto
+qed
+
+lemma signal_of2_purged:
+  assumes "k < t + dly"
+  assumes "\<And>n. n < t \<Longrightarrow> lookup \<tau>1 n = 0"
+  assumes "\<And>s. s \<in> dom (lookup \<tau>1 t) \<Longrightarrow> \<sigma> s = the (lookup \<tau>1 t s)"
+  shows "signal_of2 (\<sigma> sig) (purge dly \<tau>1 t sig (\<sigma> sig)) sig k = (\<sigma> sig)"
+proof -
+  have *: "\<And>k. k \<le> t \<Longrightarrow> lookup (purge dly \<tau>1 t sig (\<sigma> sig)) k = lookup \<tau>1 k"
+    by (transfer', metis purge_raw_before_now_unchanged)
+  have **: "\<And>k. k < t \<Longrightarrow> lookup (purge dly \<tau>1 t sig (\<sigma> sig)) k = 0"
+    using assms(2) * by auto
+  have "k < t \<or> k = t \<or> t < k"
+    by auto
+  moreover
+  { assume "k < t "
+    have ?thesis
+    proof -
+      have "\<forall>n\<in>dom (lookup (to_transaction2 (purge dly \<tau>1 t sig (\<sigma> sig)) sig)). k < n"
+      proof (rule ccontr)
+        assume "\<not> (\<forall>n\<in>dom (lookup (to_transaction2 (purge dly \<tau>1 t sig (\<sigma> sig)) sig)). k < n)"
+        then obtain n where "n \<in> dom (lookup (to_transaction2 (purge dly \<tau>1 t sig (\<sigma> sig)) sig))"
+          and "n \<le> k"  using not_less by blast
+        with `k < t` have "n < t" by auto
+        hence " lookup (purge dly \<tau>1 t sig (\<sigma> sig)) n = lookup \<tau>1 n "
+          using * by auto
+        also have "... = 0"
+          using assms(2) `n < t` by auto
+        finally have "lookup (purge dly \<tau>1 t sig (\<sigma> sig)) n = 0"
+          by auto
+        hence "n \<notin> dom (lookup (to_transaction2 (purge dly \<tau>1 t sig (\<sigma> sig)) sig))"
+          apply transfer' unfolding to_trans_raw2_def 
+          by (simp add: domIff zero_fun_def zero_option_def)
+        with `n \<in> dom (lookup (to_transaction2 (purge dly \<tau>1 t sig (\<sigma> sig)) sig))`
+        show False by auto
+      qed
+      hence "inf_time (to_transaction2 (purge dly \<tau>1 t sig (\<sigma> sig))) sig k = None"
+        by (rule inf_time_noneI)
+      thus ?thesis
+        unfolding to_signal2_def comp_def by auto
+    qed }
+  moreover
+  { assume "k = t"
+    hence "lookup (purge dly \<tau>1 t sig (\<sigma> sig)) k sig = lookup \<tau>1 k sig"
+      by (transfer', metis less_or_eq_imp_le purge_raw_before_now_unchanged)
+    obtain x where "lookup \<tau>1 k sig = None \<or> lookup \<tau>1 k sig = Some x"
+      by (meson not_None_eq)
+    moreover
+    { assume "lookup \<tau>1 k sig = None"
+      have ?thesis
+      proof -
+        have "\<forall>n\<in>dom (lookup (to_transaction2 (purge dly \<tau>1 t sig (\<sigma> sig)) sig)). k < n"
+        proof (rule ccontr)
+          assume "\<not> (\<forall>n\<in>dom (lookup (to_transaction2 (purge dly \<tau>1 t sig (\<sigma> sig)) sig)). k < n)"
+          then obtain n where "n \<in> dom (lookup (to_transaction2 (purge dly \<tau>1 t sig (\<sigma> sig)) sig))"
+            and "n \<le> k"  using not_less by blast
+          with `k = t` have "n \<le> t" by auto
+          hence " lookup (purge dly \<tau>1 t sig (\<sigma> sig)) n sig = lookup \<tau>1 n sig"
+            using * by auto
+          also have "... = 0"
+            using assms(2) `n \<le> t` `lookup \<tau>1 k sig = None` 
+            by (metis \<open>k = t\<close> dual_order.order_iff_strict zero_fun_def zero_option_def)
+          finally have "lookup (purge dly \<tau>1 t sig (\<sigma> sig)) n sig = 0"
+            by auto
+          hence "n \<notin> dom (lookup (to_transaction2 (purge dly \<tau>1 t sig (\<sigma> sig)) sig))"
+            apply transfer' unfolding to_trans_raw2_def 
+            by (simp add: domIff zero_fun_def zero_option_def)
+          with `n \<in> dom (lookup (to_transaction2 (purge dly \<tau>1 t sig (\<sigma> sig)) sig))`
+          show False by auto
+        qed
+        hence "inf_time (to_transaction2 (purge dly \<tau>1 t sig (\<sigma> sig))) sig k = None"
+          by (rule inf_time_noneI)
+        thus ?thesis
+          unfolding to_signal2_def comp_def by auto
+      qed }
+    moreover
+    { assume "lookup \<tau>1 k sig = Some x"
+      hence "x = \<sigma> sig"
+        using assms(3)  by (simp add: \<open>k = t\<close> domIff)
+      hence "lookup \<tau>1 k sig = Some (\<sigma> sig)"
+        using `lookup \<tau>1 k sig = Some x` by auto
+      hence ?thesis
+        using \<open>get_trans (purge dly \<tau>1 t sig (\<sigma> sig)) k sig = get_trans \<tau>1 k sig\<close> lookup_some_signal_of2' 
+        by fastforce }
+    ultimately have ?thesis by auto }
+  moreover
+  { assume "t < k"  
+    have "lookup (purge dly \<tau>1 t sig (\<sigma> sig)) k sig = None \<or> 
+          lookup (purge dly \<tau>1 t sig (\<sigma> sig)) k sig = Some (\<sigma> sig)"
+      by (simp add: \<open>t < k\<close> assms(1) order.strict_implies_order purge_correctness')    
+    moreover
+    { assume "lookup (purge dly \<tau>1 t sig (\<sigma> sig)) k sig = Some (\<sigma> sig)"
+      hence ?thesis
+        by (meson lookup_some_signal_of2') }
+    moreover
+    { assume "lookup (purge dly \<tau>1 t sig (\<sigma> sig)) k sig = None"
+      define \<tau>1' where "\<tau>1' = purge dly \<tau>1 t sig (\<sigma> sig)"
+      obtain k' where "find (\<lambda>x. lookup \<tau>1' x sig \<noteq> None) (rev [0..< k]) = None \<or>
+                       find (\<lambda>x. lookup \<tau>1' x sig \<noteq> None) (rev [0..< k]) = Some k'"
+        using option.exhaust_sel by blast
+      moreover
+      { assume "find (\<lambda>x. lookup \<tau>1' x sig \<noteq> None) (rev [0..< k]) = None"
+        hence "\<not> (\<exists>x. x \<in> set [0 ..< k] \<and> lookup \<tau>1' x sig \<noteq> None)"
+          unfolding find_None_iff by auto
+        hence "\<And>x. x < k \<Longrightarrow> lookup \<tau>1' x sig = None"
+          by auto
+        hence ***: "\<And>x. x \<le> k \<Longrightarrow> lookup \<tau>1' x sig = None"
+          using `lookup (purge dly \<tau>1 t sig (\<sigma> sig)) k sig = None` 
+          unfolding \<tau>1'_def using nat_less_le by blast
+        have "signal_of2 (\<sigma> sig) \<tau>1' sig k = \<sigma> sig"
+        proof -
+          have "\<forall>t\<in>dom (lookup (to_transaction2 \<tau>1' sig)). k < t"
+          proof (rule ccontr)
+            assume "\<not>(\<forall>t\<in>dom (lookup (to_transaction2 \<tau>1' sig)). k < t)"
+            then obtain t where "t \<in>dom (lookup (to_transaction2 \<tau>1' sig))" and "t \<le> k"
+              using leI by blast
+            with *** have "lookup \<tau>1' t sig = None"
+              by auto
+            hence "t \<notin> dom (lookup (to_transaction2 \<tau>1' sig))"
+              apply transfer' unfolding to_trans_raw2_def by auto
+            thus False
+              using \<open>t \<in> dom (lookup (to_transaction2 \<tau>1' sig))\<close> by blast
+          qed
+          hence " inf_time (to_transaction2 \<tau>1') sig k = None"
+            by (rule inf_time_noneI)
+          thus ?thesis
+            unfolding to_signal2_def comp_def by auto
+        qed
+        hence ?thesis
+          unfolding \<tau>1'_def by auto }
+      moreover
+      { assume "find (\<lambda>x. lookup \<tau>1' x sig \<noteq> None) (rev [0..< k]) = Some k'"
+        hence " \<exists>i<length (rev [0..<k]). get_trans \<tau>1' (rev [0..<k] ! i) sig \<noteq> None 
+                                       \<and> k' = rev [0..<k] ! i 
+                                       \<and> (\<forall>j<i. \<not> get_trans \<tau>1' (rev [0..<k] ! j) sig \<noteq> None)"
+          unfolding find_Some_iff by auto
+        then obtain i where "i<length (rev [0..<k])" and "get_trans \<tau>1' (rev [0..<k] ! i) sig \<noteq> None"
+                      and "k' = rev [0..<k] ! i " and quant: "\<forall>j<i.  lookup \<tau>1' (rev [0..<k] ! j) sig = None"
+          by auto
+        have "k' = k - i - 1" using `k' = rev [0..<k] ! i` 
+          by (metis One_nat_def \<open>i < length (rev [0..<k])\<close> add.left_neutral add.right_neutral 
+              add_Suc_right diff_diff_add diff_less diff_zero length_rev length_upt nat_less_le 
+              neq0_conv nth_upt rev_nth zero_less_Suc zero_order(2))
+        hence iless: "i < length ([0..<k])"
+          using `i<length (rev [0..<k])` by auto
+        have "lookup \<tau>1' k' sig \<noteq> None" 
+          using rev_nth[OF iless] `lookup \<tau>1' (rev [0..<k] ! i) sig \<noteq> None` `k' = k - i - 1`
+          using \<open>k' = rev [0..<k] ! i\<close> by auto
+        have "\<And>j. j > k' \<Longrightarrow>  j < k \<Longrightarrow> lookup \<tau>1' j sig = None"
+        proof -
+          fix j
+          assume "k'< j" and "j < k"
+          define j' where "j' = k - j - 1"
+          have "k - i - 1 < j"
+            using `k'< j` unfolding `k' = k - i - 1` by auto
+          hence "j' < i"
+            unfolding j'_def  using `j < k` by linarith
+          hence lookup: "lookup \<tau>1' (rev [0..< k] ! j') sig = None"
+            using quant by auto
+          have "j' < k"
+            unfolding j'_def using `j < k` by auto
+          with rev_nth have "rev [0 ..< k] ! j' = [0 ..< k] ! j"
+            unfolding j'_def  by (simp add: rev_nth Suc_diff_Suc \<open>j < k\<close> less_imp_le_nat)
+          with lookup have "get_trans \<tau>1' ([0 ..< k] ! j) sig = None"
+            by auto
+          thus "get_trans \<tau>1' j sig = None"
+            using nth_upt `j < k` by auto
+        qed
+        hence ind: "\<And>j. k' < j \<Longrightarrow> j \<le> k \<Longrightarrow> lookup \<tau>1' j sig = 0"
+          using `lookup (purge dly \<tau>1 t sig (\<sigma> sig)) k sig = None` unfolding \<tau>1'_def 
+          using dual_order.order_iff_strict  zero_option_def by fastforce
+        have "k' < k"
+          using \<open>i < length (rev [0..<k])\<close> \<open>k' = k - i - 1\<close> by auto
+        hence " signal_of2 (\<sigma> sig) \<tau>1' sig k = signal_of2 (\<sigma> sig) \<tau>1' sig k'"
+          using signal_of2_less_ind'[OF ind `k' < k`] by auto
+        have "t \<le> k'"
+        proof (rule ccontr)
+          assume "\<not> t \<le> k'" hence "k' < t" by auto
+          have "lookup \<tau>1' k' sig = lookup \<tau>1 k' sig"
+            unfolding \<tau>1'_def by (simp add: "**" \<open>k' < t\<close> assms(2))
+          also have "... = 0"
+            using assms(2) `k' < t` by (simp add: zero_fun_def)
+          finally have "lookup \<tau>1' k' sig = 0"
+            by auto
+          with `lookup \<tau>1' k' sig \<noteq> None` show False  by (simp add: zero_option_def)
+        qed
+        hence "t \<noteq> k' \<or> t = k'" by auto
+        moreover
+        { assume "t \<noteq> k'"
+          hence "lookup \<tau>1' k' sig = Some (\<sigma> sig)"
+            unfolding \<tau>1'_def using `k' < k` `k < t + dly` `t \<le> k'` `lookup \<tau>1' k' sig \<noteq> None`
+            by (metis (no_types, lifting) \<tau>1'_def le_cases le_less_trans le_neq_trans less_irrefl purge_correctness')
+          hence "signal_of2 (\<sigma> sig) \<tau>1' sig k' = \<sigma> sig"
+            by (meson lookup_some_signal_of2')
+          with `signal_of2 (\<sigma> sig) \<tau>1' sig k = signal_of2 (\<sigma> sig) \<tau>1' sig k'`
+          have ?thesis unfolding \<tau>1'_def by auto }
+        moreover
+        { assume "t = k'"
+          have "lookup \<tau>1' k' sig = lookup \<tau>1 k' sig"
+            using `t = k'` * unfolding \<tau>1'_def by auto
+          obtain m where "lookup \<tau>1 k' sig = None \<or> lookup \<tau>1 k' sig = Some m"
+            by (meson not_Some_eq)
+          moreover
+          { assume "lookup \<tau>1 k' sig = Some m"
+            hence "m = \<sigma> sig"
+              using `t = k'` assms(3) by (simp add: domIff)
+            hence "lookup \<tau>1 k' sig = Some (\<sigma> sig)"
+              using `lookup \<tau>1 k' sig = Some m` by auto
+            hence "lookup \<tau>1' k' sig = Some (\<sigma> sig)"
+              using `lookup \<tau>1' k' sig = lookup \<tau>1 k' sig` by auto
+            hence "signal_of2 (\<sigma> sig) \<tau>1' sig k' = \<sigma> sig"
+              by (meson lookup_some_signal_of2')
+            hence ?thesis
+              using `signal_of2 (\<sigma> sig) \<tau>1' sig k = signal_of2 (\<sigma> sig) \<tau>1' sig k'`
+              unfolding \<tau>1'_def by auto }
+          moreover
+          { assume "lookup \<tau>1 k' sig = None"
+            hence "lookup \<tau>1' k' sig = None"
+              using `lookup \<tau>1' k' sig = lookup \<tau>1 k' sig` by auto
+            hence "signal_of2 (\<sigma> sig) \<tau>1' sig k = \<sigma> sig"
+            proof -
+              have "\<forall>n\<in>dom (lookup (to_transaction2 \<tau>1' sig)). k < n"
+              proof (rule ccontr)
+                assume "\<not> (\<forall>n\<in>dom (lookup (to_transaction2 \<tau>1' sig)). k < n)"
+                then obtain n where "n \<in> dom (lookup (to_transaction2 \<tau>1' sig))" and "n \<le> k"
+                  using \<open>get_trans \<tau>1' k' sig = None\<close> \<open>get_trans \<tau>1' k' sig \<noteq> None\<close> by blast
+                have "lookup \<tau>1' n sig = None"
+                  using `n \<le> k` ** `lookup \<tau>1' k' sig = None` `t = k'` unfolding \<tau>1'_def 
+                  using \<open>get_trans \<tau>1' k' sig \<noteq> None\<close> \<tau>1'_def by blast
+                hence "n \<notin> dom (lookup (to_transaction2 \<tau>1' sig))"
+                  by (transfer', auto simp add:to_trans_raw2_def) 
+                with `n \<in> dom (lookup (to_transaction2 \<tau>1' sig))` show False 
+                  by auto
+              qed
+              hence "inf_time (to_transaction2 \<tau>1') sig k = None "
+                by (rule inf_time_noneI)
+              thus ?thesis
+                unfolding to_signal2_def comp_def by auto
+            qed
+            hence ?thesis
+              unfolding \<tau>1'_def by auto }
+          ultimately have ?thesis by auto }
+        ultimately have ?thesis by auto }
+      ultimately have ?thesis by auto }
+    ultimately have ?thesis by auto }
+  ultimately show ?thesis by auto
+qed
+         
+lemma helper':
+  assumes "t, \<sigma>, \<gamma>, \<theta>1 \<turnstile> <ss, \<tau>1> \<longrightarrow>\<^sub>s \<tau>1'"
+  assumes "\<And>k s. signal_of2 False \<theta>1 s k = signal_of2 False \<theta>2 s k"
+  assumes "\<And>k s. signal_of2 (\<sigma> s) \<tau>1 s k = signal_of2 (\<sigma> s) \<tau>2 s k"
+  assumes "t, \<sigma>, \<gamma>, \<theta>2 \<turnstile> <ss, \<tau>2> \<longrightarrow>\<^sub>s \<tau>2'"
+  assumes "context_invariant t \<sigma> \<gamma> \<theta>1 \<tau>1" and "context_invariant t \<sigma> \<gamma> \<theta>2 \<tau>2"
+  assumes "nonneg_delay ss"
+  shows "\<And>k s. signal_of2 (\<sigma> s) \<tau>1' s k = signal_of2 (\<sigma> s) \<tau>2' s k"
+  using assms
+proof (induction ss arbitrary:\<tau>1 \<tau>2 \<tau>1' \<tau>2')
+  case (Bcomp ss1 ss2)
+  then obtain \<tau> \<tau>' where tau1: "t , \<sigma> , \<gamma> , \<theta>1 \<turnstile> <ss1, \<tau>1> \<longrightarrow>\<^sub>s \<tau>" and tau2: "t , \<sigma> , \<gamma> , \<theta>1 \<turnstile> <ss2 , \<tau>> \<longrightarrow>\<^sub>s \<tau>1'"
+      and tau3: "t , \<sigma> , \<gamma> , \<theta>2 \<turnstile> <ss1, \<tau>2> \<longrightarrow>\<^sub>s \<tau>'" and tau4: "t , \<sigma> , \<gamma> , \<theta>2 \<turnstile> <ss2 , \<tau>'> \<longrightarrow>\<^sub>s \<tau>2'"
+      and "nonneg_delay ss1" and "nonneg_delay ss2"
+    by auto
+  have "\<And>k s. signal_of2 (\<sigma> s) \<tau> s k = signal_of2 (\<sigma> s) \<tau>' s k"
+    using Bcomp(1)[OF tau1 Bcomp(4) Bcomp(5) tau3 Bcomp(7-8) `nonneg_delay ss1`] by auto
+  moreover have "context_invariant t \<sigma> \<gamma> \<theta>1 \<tau>"
+    using b_seq_exec_preserves_context_invariant[OF Bcomp(7) tau1 `nonneg_delay ss1`] 
+    by auto
+  moreover have "context_invariant t \<sigma> \<gamma> \<theta>2 \<tau>'"
+    using b_seq_exec_preserves_context_invariant[OF Bcomp(8) tau3 `nonneg_delay ss1`] .
+  ultimately show ?case 
+    using Bcomp(2)[OF tau2 Bcomp(4) _ tau4] `nonneg_delay ss2` by auto
+next
+  case (Bguarded g ss1 ss2)
+  hence "nonneg_delay ss1" and "nonneg_delay ss2"
+    by auto
+  have "beval t \<sigma> \<gamma> \<theta>1 g \<or> \<not> beval t \<sigma> \<gamma> \<theta>1 g"
+    by auto
+  moreover
+  { assume "beval t \<sigma> \<gamma> \<theta>1 g"
+    hence "\<tau>1' = b_seq_exec t \<sigma> \<gamma> \<theta>1 ss1 \<tau>1"
+      using Bguarded by auto
+    have "beval t \<sigma> \<gamma> \<theta>2 g"
+      using beval_cong[OF Bguarded(4)] `beval t \<sigma> \<gamma> \<theta>1 g` by auto
+    hence "\<tau>2' = b_seq_exec t \<sigma> \<gamma> \<theta>2 ss1 \<tau>2"
+      using Bguarded(6) by auto
+    hence ?case
+      using Bguarded(1) `\<tau>1' = b_seq_exec t \<sigma> \<gamma> \<theta>1 ss1 \<tau>1` Bguarded(4-5) 
+      Bguarded.prems(5) Bguarded.prems(6) \<open>nonneg_delay ss1\<close> by blast }
+  moreover
+  { assume "\<not> beval t \<sigma> \<gamma> \<theta>1 g"
+    hence "\<not> beval t \<sigma> \<gamma> \<theta>2 g"
+      using beval_cong[OF Bguarded(4)] by auto
+    hence "\<tau>1' = b_seq_exec t \<sigma> \<gamma> \<theta>1 ss2 \<tau>1" and "\<tau>2' = b_seq_exec t \<sigma> \<gamma> \<theta>2 ss2 \<tau>2"
+      using `\<not> beval t \<sigma> \<gamma> \<theta>1 g` using Bguarded by auto
+    hence ?case 
+      using Bguarded \<open>nonneg_delay ss2\<close> by blast }
+  ultimately show ?case 
+    by auto
+next
+  case (Bassign_trans sig e dly)
+  define x where "x = (beval t \<sigma> \<gamma> \<theta>1 e)"
+  hence "x = beval t \<sigma> \<gamma> \<theta>2 e"
+    using beval_cong[OF Bassign_trans(2)] by auto
+  have tau1: "\<tau>1' = trans_post sig x \<tau>1 (t + dly)"
+    using Bassign_trans(1)  using x_def by auto
+  have tau2:  "\<tau>2' = trans_post sig x \<tau>2 (t + dly)"
+    using Bassign_trans(4) using `x = beval t \<sigma> \<gamma> \<theta>2 e`  by simp
+  have "s \<noteq> sig \<Longrightarrow> signal_of2 (\<sigma> s) \<tau>1' s k = signal_of2 (\<sigma> s) \<tau>1 s k"
+    using signal_of_trans_post unfolding tau1 by metis
+  moreover have "s \<noteq> sig \<Longrightarrow> signal_of2 (\<sigma> s) \<tau>1 s k = signal_of2 (\<sigma> s) \<tau>2 s k"
+    using Bassign_trans(3) by auto
+  ultimately have *: "s \<noteq> sig \<Longrightarrow> signal_of2 (\<sigma> s) \<tau>1' s k = signal_of2 (\<sigma> s) \<tau>2' s k"
+    using signal_of_trans_post unfolding tau2 by metis
+  have "t + dly \<le> k \<or> k < t + dly"
+    by auto
+  moreover
+  { assume "t + dly \<le> k"
+    from signal_of_trans_post3[OF this] have "signal_of2 (\<sigma> s) \<tau>1' sig k = x"
+      unfolding tau1 by metis
+    moreover from signal_of_trans_post3[OF `t + dly \<le> k`] have "signal_of2 (\<sigma> s) \<tau>2' sig k = x"
+      unfolding tau2  by metis
+    ultimately have "signal_of2 (\<sigma> s) \<tau>1' sig k = signal_of2 (\<sigma> s) \<tau>2' sig k"
+      by auto
+    with * have "signal_of2 (\<sigma> s) \<tau>1' s k = signal_of2 (\<sigma> s) \<tau>2' s k"
+      by auto }
+  moreover
+  { assume "k < t + dly"
+    from signal_of_trans_post2[OF this] have "signal_of2 (\<sigma> s) \<tau>1' sig k = signal_of2 (\<sigma> s) \<tau>1 sig k"
+      and "signal_of2 (\<sigma> s) \<tau>2' sig k = signal_of2 (\<sigma> s) \<tau>2 sig k" unfolding tau1 tau2 by metis+
+    with * have "signal_of2 (\<sigma> s) \<tau>1' s k = signal_of2 (\<sigma> s) \<tau>2' s k"
+      using Bassign_trans(3) by auto }
+  ultimately show ?case by auto
+next
+  case (Bassign_inert sig e dly)
+  define x where "x = (beval t \<sigma> \<gamma> \<theta>1 e)"
+  hence "x = beval t \<sigma> \<gamma> \<theta>2 e"
+    using beval_cong[OF Bassign_inert(2)] by auto
+  have tau1: "\<tau>1' = inr_post sig x (\<sigma> sig) \<tau>1 t dly"
+    using Bassign_inert(1)  using x_def by auto
+  have tau2:  "\<tau>2' = inr_post sig x (\<sigma> sig) \<tau>2 t dly"
+    using Bassign_inert(4) using `x = beval t \<sigma> \<gamma> \<theta>2 e`  by simp
+  have ci0: "\<And>n. n < t \<Longrightarrow> lookup \<tau>1 n = 0" and ci1: "\<And>s. s \<in> dom (lookup \<tau>1 t) \<Longrightarrow> \<sigma> s = the (lookup \<tau>1 t s)"
+    using `context_invariant t \<sigma> \<gamma> \<theta>1 \<tau>1` unfolding context_invariant_def by auto
+  have "is_stable dly \<tau>1 t sig (\<sigma> sig) \<or> \<not> is_stable dly \<tau>1 t sig (\<sigma> sig)"
+    by auto
+  moreover
+  { assume stab1: "is_stable dly \<tau>1 t sig (\<sigma> sig)" hence stab2:"is_stable dly \<tau>2 t sig (\<sigma> sig)"
+      using signal_of2_eq_is_stable[OF _ Bassign_inert(3) ci0 ci1] by auto
+    have tau1': "\<tau>1' = trans_post sig x \<tau>1 (t + dly)"
+      using stab1 tau1 unfolding inr_post_def by auto
+    moreover have tau2': "\<tau>2' = trans_post sig x \<tau>2 (t + dly)"
+      using stab2 tau2 unfolding inr_post_def by auto
+    have "t + dly \<le> k \<or> k < t + dly"
+      by auto
+    have "s \<noteq> sig \<Longrightarrow> signal_of2 (\<sigma> s) \<tau>1' s k = signal_of2 (\<sigma> s) \<tau>1 s k"
+      using signal_of_trans_post unfolding tau1' by metis
+    moreover have "s \<noteq> sig \<Longrightarrow> signal_of2 (\<sigma> s) \<tau>1 s k = signal_of2 (\<sigma> s) \<tau>2 s k"
+      using Bassign_inert(3) by auto
+    ultimately have *: "s \<noteq> sig \<Longrightarrow> signal_of2 (\<sigma> s) \<tau>1' s k = signal_of2 (\<sigma> s) \<tau>2' s k"
+      using signal_of_trans_post unfolding tau2' by metis
+    have "t + dly \<le> k \<or> k < t + dly"
+      by auto
+    moreover
+    { assume "t + dly \<le> k"
+      from signal_of_trans_post3[OF this] have "signal_of2 (\<sigma> s) \<tau>1' sig k = x"
+        unfolding tau1' by metis
+      moreover from signal_of_trans_post3[OF `t + dly \<le> k`] have "signal_of2 (\<sigma> s) \<tau>2' sig k = x"
+        unfolding tau2'  by metis
+      ultimately have "signal_of2 (\<sigma> s) \<tau>1' sig k = signal_of2 (\<sigma> s) \<tau>2' sig k"
+        by auto
+      with * have "signal_of2 (\<sigma> s) \<tau>1' s k = signal_of2 (\<sigma> s) \<tau>2' s k"
+        by auto }
+    moreover
+    { assume "k < t + dly"
+      from signal_of_trans_post2[OF this] have "signal_of2 (\<sigma> s) \<tau>1' sig k = signal_of2 (\<sigma> s) \<tau>1 sig k"
+        and "signal_of2 (\<sigma> s) \<tau>2' sig k = signal_of2 (\<sigma> s) \<tau>2 sig k" unfolding tau1' tau2' by metis+
+      with * have "signal_of2 (\<sigma> s) \<tau>1' s k = signal_of2 (\<sigma> s) \<tau>2' s k"
+        using Bassign_inert(3) by auto }
+    ultimately have ?case by auto }
+  moreover
+  { assume nstable1: "\<not> is_stable dly \<tau>1 t sig (\<sigma> sig)"
+    have ci2: "\<And>n. n < t \<Longrightarrow> lookup \<tau>2 n = 0" and ci3: "\<And>s. s \<in> dom (lookup \<tau>2 t) \<Longrightarrow> \<sigma> s = the (lookup \<tau>2 t s)"
+      using `context_invariant t \<sigma> \<gamma> \<theta>2 \<tau>2` unfolding context_invariant_def by auto
+    have nstable2: "\<not> is_stable dly \<tau>2 t sig (\<sigma> sig)"
+      using signal_of2_eq_is_stable_eq[OF ci0 ci1 ci2 ci3 Bassign_inert(3)] 
+      `\<not> is_stable dly \<tau>1 t sig (\<sigma> sig)` by auto
+    have tau1': "\<tau>1' = trans_post sig x (purge dly \<tau>1 t sig (\<sigma> sig)) (t + dly)"
+      using tau1 nstable1 unfolding inr_post_def by auto
+    have tau2': "\<tau>2' = trans_post sig x (purge dly \<tau>2 t sig (\<sigma> sig)) (t + dly)"
+      using tau2 nstable2 unfolding inr_post_def by auto
+    have "t + dly \<le> k \<or> k < t + dly"
+      by auto
+    have "s \<noteq> sig \<Longrightarrow> signal_of2 (\<sigma> s) \<tau>1' s k = signal_of2 (\<sigma> s) (purge dly \<tau>1 t sig (\<sigma> sig)) s k"
+      using signal_of_trans_post unfolding tau1' by metis
+    moreover have "s \<noteq> sig \<Longrightarrow> signal_of2 (\<sigma> s) (purge dly \<tau>1 t sig (\<sigma> sig)) s k = signal_of2 (\<sigma> s) \<tau>1 s k"
+      using signal_of2_purge_not_affected  by fastforce
+    moreover have "s \<noteq> sig \<Longrightarrow> signal_of2 (\<sigma> s) \<tau>1 s k = signal_of2 (\<sigma> s) \<tau>2 s k"
+      using Bassign_inert(3) by auto
+    moreover have "s \<noteq> sig \<Longrightarrow> signal_of2 (\<sigma> s) \<tau>2 s k = signal_of2 (\<sigma> s) (purge dly \<tau>2 t sig (\<sigma> sig)) s k"
+      using signal_of2_purge_not_affected by fastforce
+    ultimately have *: "s \<noteq> sig \<Longrightarrow> signal_of2 (\<sigma> s) \<tau>1' s k = signal_of2 (\<sigma> s) \<tau>2' s k"
+      using signal_of_trans_post unfolding tau2' by metis    
+    have "t + dly \<le> k \<or> k < t + dly"
+      by auto
+    moreover
+    { assume "t + dly \<le> k"
+      from signal_of_trans_post3[OF this] have "signal_of2 (\<sigma> s) \<tau>1' sig k = x"
+        unfolding tau1' by metis
+      moreover from signal_of_trans_post3[OF `t + dly \<le> k`] have "signal_of2 (\<sigma> s) \<tau>2' sig k = x"
+        unfolding tau2'  by metis
+      ultimately have "signal_of2 (\<sigma> s) \<tau>1' sig k = signal_of2 (\<sigma> s) \<tau>2' sig k"
+        by auto
+      with * have "signal_of2 (\<sigma> s) \<tau>1' s k = signal_of2 (\<sigma> s) \<tau>2' s k"
+        by auto }
+    moreover
+    { assume "k < t + dly"
+      from signal_of_trans_post2[OF this] have "signal_of2 (\<sigma> sig) \<tau>1' sig k = signal_of2 (\<sigma> sig) (purge dly \<tau>1 t sig (\<sigma> sig)) sig k"
+        and "signal_of2 (\<sigma> sig) \<tau>2' sig k = signal_of2 (\<sigma> sig) (purge dly \<tau>2 t sig (\<sigma> sig)) sig k" unfolding tau1' tau2' by metis+
+      moreover have "signal_of2 (\<sigma> sig) (purge dly \<tau>1 t sig (\<sigma> sig)) sig k = \<sigma> sig"
+        using signal_of2_purged[OF `k < t + dly` `\<And>n. n < t \<Longrightarrow> get_trans \<tau>1 n = 0`
+        `\<And>s. s \<in> dom (get_trans \<tau>1 t) \<Longrightarrow> \<sigma> s = the (get_trans \<tau>1 t s)`] by auto
+      moreover have "signal_of2 (\<sigma> sig) (purge dly \<tau>2 t sig (\<sigma> sig)) sig k = \<sigma> sig"
+        using signal_of2_purged[OF `k < t + dly` `\<And>n. n < t \<Longrightarrow> get_trans \<tau>2 n = 0`
+        `\<And>s. s \<in> dom (get_trans \<tau>2 t) \<Longrightarrow> \<sigma> s = the (get_trans \<tau>2 t s)`] by auto
+      ultimately have "signal_of2 (\<sigma> s) \<tau>1' s k = signal_of2 (\<sigma> s) \<tau>2' s k"
+        using "*" by blast }
+    ultimately have "signal_of2 (\<sigma> s) \<tau>1' s k = signal_of2 (\<sigma> s) \<tau>2' s k"
+      by auto }
+  ultimately show "signal_of2 (\<sigma> s) \<tau>1' s k = signal_of2 (\<sigma> s) \<tau>2' s k"
+    by auto
+next
+  case Bnull
+  then show ?case by auto
+qed
+
+lemma helper:
+  assumes "t, \<sigma>, \<gamma>, \<theta>1 \<turnstile> <ss, \<tau>1> \<longrightarrow>\<^sub>s \<tau>1'"
+  assumes "\<And>k s. signal_of2 False \<theta>1 s k = signal_of2 False \<theta>2 s k"
+  assumes "\<And>k s. signal_of2 (\<sigma> s) \<tau>1 s k = signal_of2 (\<sigma> s) \<tau>2 s k"
+  assumes "context_invariant t \<sigma> \<gamma> \<theta>1 \<tau>1" and "context_invariant t \<sigma> \<gamma> \<theta>2 \<tau>2"
+  assumes "nonneg_delay ss"
+  shows "\<exists>\<tau>2'. (t, \<sigma>, \<gamma>, \<theta>2 \<turnstile> <ss, \<tau>2> \<longrightarrow>\<^sub>s \<tau>2') \<and> (\<forall>k s. signal_of2 (\<sigma> s) \<tau>1' s k = signal_of2 (\<sigma> s) \<tau>2' s k)"
+  using helper'[OF assms(1-3) _ assms(4-5) `nonneg_delay ss`] by auto 
+
+lemma Bcomp_hoare_valid':
+  assumes "\<Turnstile>\<^sub>t [P] s1 [Q]" and "\<Turnstile>\<^sub>t [Q] s2 [R]"
+  assumes "nonneg_delay (Bcomp s1 s2)"
+  shows "\<Turnstile>\<^sub>t [P] Bcomp s1 s2 [R]"
+  unfolding seq_hoare_valid2_def
+proof (rule)+
+  fix w w'
+  have "nonneg_delay s1" and "nonneg_delay s2"
+    using assms(3) by auto
+  assume "P w \<and> (w, t, Bcomp s1 s2 \<Rightarrow>\<^sub>s w')"
+  hence "P w" and "w, t, Bcomp s1 s2 \<Rightarrow>\<^sub>s w'" by auto
+  then obtain \<sigma> \<gamma> \<theta> \<tau> \<tau>' where des: "destruct_worldline w t = (\<sigma>, \<gamma>, \<theta>, \<tau>)" and 
+    "(t, \<sigma>, \<gamma>, \<theta> \<turnstile> <Bcomp s1 s2, \<tau>> \<longrightarrow>\<^sub>s \<tau>')" and "w'= worldline2 t \<sigma> \<theta> \<tau>'"
+    unfolding world_seq_exec_def Let_def using destruct_worldline_exist by fastforce
+  then obtain \<tau>'' where tau1: "(t, \<sigma>, \<gamma>, \<theta> \<turnstile> <s1, \<tau>> \<longrightarrow>\<^sub>s \<tau>'')" and tau2: "(t, \<sigma>, \<gamma>, \<theta> \<turnstile> <s2, \<tau>''> \<longrightarrow>\<^sub>s \<tau>')"
+    by auto
+  define w'' where "w'' = worldline2 t \<sigma> \<theta> \<tau>''"
+  hence "w, t, s1 \<Rightarrow>\<^sub>s w''"
+    using des tau1 unfolding world_seq_exec_def Let_def by auto
+  with assms(1) have "Q w''" 
+    unfolding seq_hoare_valid2_def using `P w` by auto
+  have "context_invariant t \<sigma> \<gamma> \<theta> \<tau>"
+    using worldline2_constructible[OF des] by auto
+  hence "context_invariant t \<sigma> \<gamma> \<theta> \<tau>''"
+    using b_seq_exec_preserves_context_invariant[OF _ tau1] assms(3) by auto
+  obtain \<theta>''' \<tau>''' where des2: "destruct_worldline w'' t = (\<sigma>, \<gamma>, \<theta>''', \<tau>''')" and 
+    sig_beh: "\<And>k s. signal_of2 False \<theta> s k = signal_of2 False \<theta>''' s k" and 
+    sig_trans: "\<And>k s. signal_of2 (\<sigma> s) \<tau>'' s k = signal_of2 (\<sigma> s) \<tau>''' s k"
+    unfolding w''_def using destruct_worldline_correctness[OF `context_invariant t \<sigma> \<gamma> \<theta> \<tau>''`]   
+    by (metis destruct_worldline_exist)
+  have "context_invariant t \<sigma> \<gamma> \<theta>''' \<tau>'''"
+    using worldline2_constructible[OF des2] by auto
+  then obtain \<tau>4 where tau3: "t, \<sigma>, \<gamma>, \<theta>''' \<turnstile> <s2, \<tau>'''> \<longrightarrow>\<^sub>s \<tau>4" and
+    sig_trans: "\<And>k s. signal_of2 (\<sigma> s) \<tau>4 s k = signal_of2 (\<sigma> s) \<tau>' s k"
+    using helper[OF tau2 sig_beh sig_trans `context_invariant t \<sigma> \<gamma> \<theta> \<tau>''`]  \<open>nonneg_delay s2\<close> by blast
+  have "worldline2 t \<sigma> \<theta> \<tau>' = worldline2 t \<sigma> \<theta>''' \<tau>4"
+    using sig_beh sig_trans
+  proof transfer'
+    fix \<theta>  \<theta>''' :: "'a transaction" 
+    fix \<sigma> :: "'a state" 
+    fix \<tau>'' \<tau>''' \<tau>4 t \<tau>'
+    assume 1: "\<And>s k. signal_of2 False \<theta> s k = signal_of2 False \<theta>''' s k"
+    assume  "\<And>s k. signal_of2 (\<sigma> s) \<tau>4 s k = signal_of2 (\<sigma> s) \<tau>' s k"
+    thus " worldline t \<sigma> \<theta> \<tau>' = worldline t \<sigma> \<theta>''' \<tau>4"
+      unfolding worldline_def using 1 by auto
+  qed
+  hence "w'', t, s2 \<Rightarrow>\<^sub>s w'"
+    unfolding world_seq_exec_def using des2 tau3 `w'= worldline2 t \<sigma> \<theta> \<tau>'` by auto
+  with `Q w''` show "R w'"
+    using assms(2) unfolding seq_hoare_valid2_def by auto
+qed
+  
+lemma Bnull_sound_hoare2:
+  "\<turnstile>\<^sub>t [P] Bnull [Q] \<Longrightarrow> \<Turnstile>\<^sub>t [P] Bnull [Q]"
+  by (auto dest!: BnullE'_hoare2 worldline2_constructible  simp add: seq_hoare_valid2_def world_seq_exec_def  
+      split: prod.splits)
+
+lemma Bguarded_hoare_valid2:
+  assumes "\<Turnstile>\<^sub>t [\<lambda>a. P a \<and> beval_world2 a t g] s1 [Q]" and "\<Turnstile>\<^sub>t [\<lambda>a. P a \<and> \<not> beval_world2 a t g] s2 [Q]"
+  shows "\<Turnstile>\<^sub>t [P] Bguarded g s1 s2 [Q]"
+  unfolding seq_hoare_valid2_def
+proof (rule)+
+  fix w w'
+  assume "P w \<and> (w, t, Bguarded g s1 s2 \<Rightarrow>\<^sub>s w')"
+  hence "P w" and "w, t, Bguarded g s1 s2 \<Rightarrow>\<^sub>s w'" by auto
+  obtain \<sigma> \<gamma> \<theta> \<tau> where "destruct_worldline w t = (\<sigma>, \<gamma>, \<theta>, \<tau>)"
+    by (meson destruct_worldline_def)
+  hence "w = worldline2 t \<sigma> \<theta> \<tau> " and "context_invariant t \<sigma> \<gamma> \<theta> \<tau>"
+    by(auto dest!: worldline2_constructible)
+  obtain \<tau>' where "t , \<sigma> , \<gamma> , \<theta> \<turnstile> <Bguarded g s1 s2, \<tau>> \<longrightarrow>\<^sub>s \<tau>'"
+    by auto
+  hence "w' = worldline2 t \<sigma> \<theta> \<tau>'"
+    using `w, t, Bguarded g s1 s2 \<Rightarrow>\<^sub>s w'` `destruct_worldline w t = (\<sigma>, \<gamma>, \<theta>, \<tau>)` 
+    unfolding world_seq_exec_def by auto
+  have "beval t \<sigma> \<gamma> \<theta> g \<or> \<not> beval t \<sigma> \<gamma> \<theta> g"
+    by auto
+  moreover
+  { assume "beval t \<sigma> \<gamma> \<theta> g"
+    hence "t, \<sigma>, \<gamma>, \<theta> \<turnstile> <s1, \<tau>> \<longrightarrow>\<^sub>s \<tau>'"
+      using `t, \<sigma>, \<gamma>, \<theta> \<turnstile> <Bguarded g s1 s2, \<tau>> \<longrightarrow>\<^sub>s \<tau>'` by auto
+    hence "beval_world2 w t g"
+      using `beval t \<sigma> \<gamma> \<theta> g` `w = worldline2 t \<sigma> \<theta> \<tau>` `context_invariant t \<sigma> \<gamma> \<theta> \<tau>`
+      by (transfer', simp add: beval_beval_world_ci)
+    have "w, t , s1 \<Rightarrow>\<^sub>s w'"
+      using `destruct_worldline w t = (\<sigma>, \<gamma>, \<theta>, \<tau>)` `t, \<sigma>, \<gamma>, \<theta> \<turnstile> <s1, \<tau>> \<longrightarrow>\<^sub>s \<tau>'`
+      `w' = worldline2 t \<sigma> \<theta> \<tau>'` unfolding world_seq_exec_def Let_def by auto 
+    with assms(1) and `P w` have "Q w'"
+      using `beval_world2 w t g` unfolding seq_hoare_valid2_def by auto }
+  moreover
+  { assume "\<not> beval t \<sigma> \<gamma> \<theta> g"
+    hence "t, \<sigma>, \<gamma>, \<theta> \<turnstile> <s2, \<tau>> \<longrightarrow>\<^sub>s \<tau>'"
+      using `t, \<sigma>, \<gamma>, \<theta> \<turnstile> <Bguarded g s1 s2, \<tau>> \<longrightarrow>\<^sub>s \<tau>'` by auto
+    hence "\<not> beval_world2 w t g"
+      using `\<not> beval t \<sigma> \<gamma> \<theta> g` `w = worldline2 t \<sigma> \<theta> \<tau>` `context_invariant t \<sigma> \<gamma> \<theta> \<tau>`
+      by (transfer', simp add: beval_beval_world_ci)
+    have "w, t, s2 \<Rightarrow>\<^sub>s w'"
+      using `destruct_worldline w t = (\<sigma>, \<gamma>, \<theta>, \<tau>)` `t, \<sigma>, \<gamma>, \<theta> \<turnstile> <s2, \<tau>> \<longrightarrow>\<^sub>s \<tau>'`
+      `w' = worldline2 t \<sigma> \<theta> \<tau>'` unfolding world_seq_exec_def Let_def by auto     
+    with assms(2) and `P w` have "Q w'"
+      using `\<not> beval_world2 w t g` unfolding seq_hoare_valid2_def by auto }
+  ultimately show "Q w'"
+    by auto
+qed
+
+lemma lift_world_trans_worldline_upd2:
+  assumes "w, t, Bassign_trans sig exp dly \<Rightarrow>\<^sub>s w'"
+  shows "w' = w[sig, t + dly :=\<^sub>2 beval_world2 w t exp]"
+  using assms 
+proof transfer'
+  fix w t sig 
+  fix exp :: "'a bexp" 
+  fix dly w'
+  assume "w, t , Bassign_trans sig exp dly \<Rightarrow>\<^sub>s w'"
+  obtain \<sigma> \<gamma> \<theta> \<tau> where "destruct_worldline w t = (\<sigma>, \<gamma>, \<theta>, \<tau>)"
+    by (meson destruct_worldline_def)
+  hence w_def: "w = worldline2 t \<sigma> \<theta> \<tau> " and "context_invariant t \<sigma> \<gamma> \<theta> \<tau>"
+    by(auto dest!: worldline2_constructible)
+  obtain \<tau>' where "t , \<sigma> , \<gamma> , \<theta> \<turnstile> <Bassign_trans sig exp dly, \<tau>> \<longrightarrow>\<^sub>s \<tau>'"
+    and "\<tau>' = trans_post sig (beval t \<sigma> \<gamma> \<theta> exp) \<tau> (t + dly)"
+    by auto
+  moreover have "beval t \<sigma> \<gamma> \<theta> exp = beval_world2 w t exp"
+    using `w = worldline2 t \<sigma> \<theta> \<tau> ` and `context_invariant t \<sigma> \<gamma> \<theta> \<tau>`
+    by (transfer', simp add: beval_beval_world_ci)
+  ultimately have \<tau>'_def: "\<tau>' = trans_post sig (beval_world2 w t exp) \<tau> (t + dly)"
+      by auto
+  have "w' = worldline2 t \<sigma> \<theta> \<tau>'"
+    using `w, t , Bassign_trans sig exp dly \<Rightarrow>\<^sub>s w'` `destruct_worldline w t = (\<sigma>, \<gamma>, \<theta>, \<tau>)` 
+    unfolding world_seq_exec_def  using \<open>t , \<sigma> , \<gamma> , \<theta> \<turnstile> <Bassign_trans sig exp dly , \<tau>> \<longrightarrow>\<^sub>s \<tau>'\<close> 
+    by auto
+  also have "... = w[sig, t + dly:=\<^sub>2 beval_world2 w t exp]"
+    using w_def \<tau>'_def by (transfer', meson lift_trans_post_worldline_upd)
+  finally show "w' = w[sig, t + dly:=\<^sub>2 beval_world2 w t exp]"
+    by auto
+qed
+  
+lemma Bassign_trans_sound_hoare2:
+  "\<turnstile>\<^sub>t [P] Bassign_trans sig exp dly [Q] \<Longrightarrow> \<Turnstile>\<^sub>t [P] Bassign_trans sig exp dly [Q]"
+  unfolding seq_hoare_valid2_def
+proof rule+
+  fix w w'
+  assume "\<turnstile>\<^sub>t [P] Bassign_trans sig exp dly [Q]"
+  hence imp: "\<forall>w. P w \<longrightarrow> Q(w[sig, t + dly :=\<^sub>2 beval_world2 w t exp])"
+    by (auto dest!: BassignE_hoare2)
+  assume " P w \<and> (w, t , Bassign_trans sig exp dly \<Rightarrow>\<^sub>s w')"
+  hence "P w" and "w, t, Bassign_trans sig exp dly \<Rightarrow>\<^sub>s w'" by auto
+  obtain \<sigma> \<gamma> \<theta> \<tau> where "destruct_worldline w t = (\<sigma>, \<gamma>, \<theta>, \<tau>)"
+    by (meson destruct_worldline_def)
+  obtain \<tau>' where "t , \<sigma> , \<gamma> , \<theta> \<turnstile> <Bassign_trans sig exp dly, \<tau>> \<longrightarrow>\<^sub>s \<tau>'"
+    by auto
+  hence "w' = worldline2 t \<sigma> \<theta> \<tau>'"
+    using `w, t , Bassign_trans sig exp dly \<Rightarrow>\<^sub>s w'` `destruct_worldline w t = (\<sigma>, \<gamma>, \<theta>, \<tau>)` 
+    unfolding world_seq_exec_def  using \<open>t , \<sigma> , \<gamma> , \<theta> \<turnstile> <Bassign_trans sig exp dly , \<tau>> \<longrightarrow>\<^sub>s \<tau>'\<close> by auto  
+  have "w' = w[sig, t + dly :=\<^sub>2 beval_world2 w t exp]"
+    unfolding `w' = worldline2 t \<sigma> \<theta> \<tau>'` 
+    by (simp add: \<open>w' = worldline2 t \<sigma> \<theta> \<tau>'\<close> \<open>w, t , Bassign_trans sig exp dly \<Rightarrow>\<^sub>s w'\<close> lift_world_trans_worldline_upd2) 
+  with imp and `P w` have "Q(w[sig, t + dly :=\<^sub>2 beval_world2 w t exp])"
+    by auto 
+  thus "Q w'"
+    using `Q(w[sig, t + dly :=\<^sub>2 beval_world2 w t exp])` `w' = w[sig, t + dly :=\<^sub>2 beval_world2 w t exp]`
+    by auto
+qed
+ 
+lemma lift_world_inert_worldline_upd2:
+  assumes "w, t, Bassign_inert sig exp dly \<Rightarrow>\<^sub>s w'"
+  assumes "0 < dly"
+  shows "w' = w[sig, t, dly :=\<^sub>2 beval_world2 w t exp]"
+  using assms
+proof transfer'
+  fix w t sig 
+  fix exp :: "'a bexp" 
+  fix dly w'
+  assume "w, t , Bassign_inert sig exp dly \<Rightarrow>\<^sub>s w'"  
+  assume "0 < dly"
+  obtain \<sigma> \<gamma> \<theta> \<tau> where "destruct_worldline w t = (\<sigma>, \<gamma>, \<theta>, \<tau>)"
+    by (meson destruct_worldline_def)
+  hence w_def: "w = worldline2 t \<sigma> \<theta> \<tau> " and "context_invariant t \<sigma> \<gamma> \<theta> \<tau>"
+    by(auto dest!: worldline2_constructible)
+  obtain \<tau>' where "t , \<sigma> , \<gamma> , \<theta> \<turnstile> <Bassign_inert sig exp dly, \<tau>> \<longrightarrow>\<^sub>s \<tau>'"
+    and "\<tau>' = inr_post sig (beval t \<sigma> \<gamma> \<theta> exp) (\<sigma> sig) \<tau> t dly"
+    by auto
+  moreover have "beval t \<sigma> \<gamma> \<theta> exp = beval_world2 w t exp"
+    using `w = worldline2 t \<sigma> \<theta> \<tau> ` and `context_invariant t \<sigma> \<gamma> \<theta> \<tau>`
+    by (transfer', simp add: beval_beval_world_ci)
+  ultimately have \<tau>'_def: "\<tau>' = inr_post sig (beval_world2 w t exp) (\<sigma> sig) \<tau> t dly"
+    by auto
+  have "w' = worldline2 t \<sigma> \<theta> \<tau>'"
+    using `w, t , Bassign_inert sig exp dly \<Rightarrow>\<^sub>s w'` `destruct_worldline w t = (\<sigma>, \<gamma>, \<theta>, \<tau>)` 
+    unfolding world_seq_exec_def  using \<open>t , \<sigma> , \<gamma> , \<theta> \<turnstile> <Bassign_inert sig exp dly , \<tau>> \<longrightarrow>\<^sub>s \<tau>'\<close> 
+    by auto
+  also have "... = w[sig, t, dly:=\<^sub>2 beval_world2 w t exp]"
+    using `w = worldline2 t \<sigma> \<theta> \<tau>` `context_invariant t \<sigma> \<gamma> \<theta> \<tau>`
+    `t , \<sigma> , \<gamma> , \<theta> \<turnstile> <Bassign_inert sig exp dly, \<tau>> \<longrightarrow>\<^sub>s \<tau>'` `0 < dly`
+    by (transfer', simp add: lift_inr_post_worldline_upd)
+  finally show "w' = w[sig, t, dly:=\<^sub>2 beval_world2 w t exp]"
+    by auto
+qed
+
+lemma Bassign_inert_sound_hoare2:
+  assumes "0 < dly"
+  shows "\<turnstile>\<^sub>t [P] Bassign_inert sig exp dly [Q] \<Longrightarrow> \<Turnstile>\<^sub>t [P] Bassign_inert sig exp dly [Q]"
+  unfolding seq_hoare_valid2_def
+proof rule+
+  fix w w'
+  assume "\<turnstile>\<^sub>t [P] Bassign_inert sig exp dly [Q]"
+  hence imp: "\<forall>w. P w \<longrightarrow> Q(w[sig, t, dly :=\<^sub>2 beval_world2 w t exp])"
+    by (auto dest!: Bassign_inertE_hoare2)
+  assume "P w \<and> (w, t , Bassign_inert sig exp dly \<Rightarrow>\<^sub>s w')"
+  hence "P w" and "w, t , (Bassign_inert sig exp dly) \<Rightarrow>\<^sub>s w'" by auto
+  obtain \<sigma> \<gamma> \<theta> \<tau> where "destruct_worldline w t = (\<sigma>, \<gamma>, \<theta>, \<tau>)"
+    by (meson destruct_worldline_def)
+  obtain \<tau>' where "t , \<sigma> , \<gamma> , \<theta> \<turnstile> <Bassign_inert sig exp dly, \<tau>> \<longrightarrow>\<^sub>s \<tau>'"
+    by auto
+  hence "w' = worldline2 t \<sigma> \<theta> \<tau>'"
+    using `w, t , Bassign_inert sig exp dly \<Rightarrow>\<^sub>s w'` `destruct_worldline w t = (\<sigma>, \<gamma>, \<theta>, \<tau>)` 
+    unfolding world_seq_exec_def  using \<open>t , \<sigma> , \<gamma> , \<theta> \<turnstile> <Bassign_inert sig exp dly , \<tau>> \<longrightarrow>\<^sub>s \<tau>'\<close> by auto  
+  have "w' = w[sig, t, dly :=\<^sub>2 beval_world2 w t exp]"
+    by (simp add: \<open>w, t , Bassign_inert sig exp dly \<Rightarrow>\<^sub>s w'\<close> assms lift_world_inert_worldline_upd2)
+  with imp and `P w` have "Q(w[sig, t, dly :=\<^sub>2 beval_world2 w t exp])"
+    by auto 
+  thus "Q w'"
+    using `Q(w[sig, t,  dly :=\<^sub>2 beval_world2 w t exp])` `w' = w[sig, t, dly :=\<^sub>2 beval_world2 w t exp]`
+    by auto 
+qed
+
+subsection \<open>Soundness and completeness\<close>
+
+lemma soundness_hoare2:
+  assumes "\<turnstile>\<^sub>t [P] s [R]"
+  assumes "nonneg_delay s"
+  shows "\<Turnstile>\<^sub>t [P] s [R]"
+  using assms
+proof (induction rule:seq_hoare2.induct)
+  case (AssignI2 t P sig dly exp)
+  hence "0 < dly" by auto
+  then show ?case
+    using Bassign_inert_sound_hoare2[OF `0 < dly`]  using seq_hoare2.AssignI2 by fastforce
+next
+  case (Conseq2 P' P t s Q Q')
+  then show ?case  by (auto simp add: seq_hoare_valid2_def)
+qed (auto simp add: Bnull_sound_hoare2 Bassign_trans_sound_hoare2 Bcomp_hoare_valid' Bguarded_hoare_valid2)
+
+lemma  world_seq_exec_bnull:
+  "w, t, Bnull \<Rightarrow>\<^sub>s w"
+  unfolding world_seq_exec_def Let_def
+  by (metis (mono_tags, lifting) b_seq_exec.simps(1) destruct_worldline_exist old.prod.case 
+      worldline2_constructible)
+
+lemma world_seq_exec_comp:
+  assumes "nonneg_delay (Bcomp ss1 ss2)"
+  shows "w, t, (Bcomp ss1 ss2) \<Rightarrow>\<^sub>s (world_seq_exec (world_seq_exec w t ss1) t ss2)"
+proof -
+  obtain \<sigma> \<gamma> \<theta> \<tau> \<tau>' where des1: "destruct_worldline w t = (\<sigma>, \<gamma>, \<theta>, \<tau>)" and 
+    "t, \<sigma>, \<gamma>, \<theta> \<turnstile> <Bcomp ss1 ss2, \<tau>> \<longrightarrow>\<^sub>s \<tau>'" and ci1: "context_invariant t \<sigma> \<gamma> \<theta> \<tau>"
+    using destruct_worldline_exist worldline2_constructible by blast
+  then obtain \<tau>'' where "t, \<sigma>, \<gamma>, \<theta> \<turnstile> <ss1, \<tau>> \<longrightarrow>\<^sub>s \<tau>''" and exec1: "t, \<sigma>, \<gamma>, \<theta> \<turnstile> <ss2, \<tau>''> \<longrightarrow>\<^sub>s \<tau>'"
+    and ci2: "context_invariant t \<sigma> \<gamma> \<theta> \<tau>''" using b_seq_exec_preserves_context_invariant
+    using assms by fastforce
+  hence *: "worldline2 t \<sigma> \<theta> \<tau>'' = world_seq_exec w t ss1"
+    unfolding world_seq_exec_def Let_def using des1 by auto
+
+  obtain \<theta>2 \<tau>2 \<tau>3 where des2: "destruct_worldline (worldline2 t \<sigma> \<theta> \<tau>'') t = (\<sigma>, \<gamma>, \<theta>2, \<tau>2)" and 
+    beh_same:"\<And>s k. signal_of2 False \<theta> s k = signal_of2 False \<theta>2 s k" and 
+    trans_same: "\<And>s k. signal_of2 (\<sigma> s) \<tau>'' s k = signal_of2 (\<sigma> s) \<tau>2 s k" and 
+    exec2: "t, \<sigma>, \<gamma>, \<theta>2 \<turnstile> <ss2, \<tau>2> \<longrightarrow>\<^sub>s \<tau>3" 
+    using destruct_worldline_correctness[OF ci2]  by (metis prod.exhaust_sel)
+  have ci3: "context_invariant t \<sigma> \<gamma> \<theta>2 \<tau>2"
+    using worldline2_constructible[OF des2] by auto
+  have "\<And>s k. signal_of2 (\<sigma> s) \<tau>' s k = signal_of2 (\<sigma> s) \<tau>3 s k"
+    using helper'[OF exec1 beh_same trans_same exec2 ci2 ci3] assms by auto
+  hence "worldline2 t \<sigma> \<theta> \<tau>' = worldline2 t \<sigma> \<theta>2 \<tau>3"
+    using beh_same 
+  proof (transfer')
+    fix \<sigma> :: "'a state"
+    fix \<tau>' \<tau>3 
+    fix \<theta> \<theta>2 :: "'a transaction" 
+    fix t
+    assume 1: "\<And>s k. signal_of2 (\<sigma> s) \<tau>' s k = signal_of2 (\<sigma> s) \<tau>3 s k"
+    assume "\<And>s k. signal_of2 False \<theta> s k = signal_of2 False \<theta>2 s k"
+    thus " worldline t \<sigma> \<theta> \<tau>' = worldline t \<sigma> \<theta>2 \<tau>3 "
+      unfolding worldline_def  using 1 by auto
+  qed
+  also have "... = world_seq_exec (worldline2 t \<sigma> \<theta> \<tau>'') t ss2"
+    using des2 `t, \<sigma>, \<gamma>, \<theta>2 \<turnstile> <ss2, \<tau>2> \<longrightarrow>\<^sub>s \<tau>3` unfolding world_seq_exec_def Let_def 
+    by auto
+  finally have "worldline2 t \<sigma> \<theta> \<tau>' = world_seq_exec (worldline2 t \<sigma> \<theta> \<tau>'') t ss2"
+    by auto
+  thus ?thesis
+    using des1 `t, \<sigma>, \<gamma>, \<theta> \<turnstile> <Bcomp ss1 ss2, \<tau>> \<longrightarrow>\<^sub>s \<tau>'` unfolding  *
+    world_seq_exec_def Let_def by auto
+qed
+
+lemma world_seq_exec_guarded:
+  assumes "beval_world2 w t g"
+  shows "world_seq_exec w t (Bguarded g ss1 ss2) = world_seq_exec w t ss1"
+proof -
+  obtain \<sigma> \<gamma> \<theta> \<tau> \<tau>' where des1: "destruct_worldline w t = (\<sigma>, \<gamma>, \<theta>, \<tau>)" and 
+    "t, \<sigma>, \<gamma>, \<theta> \<turnstile> <Bguarded g ss1 ss2, \<tau>> \<longrightarrow>\<^sub>s \<tau>'" and ci1: "context_invariant t \<sigma> \<gamma> \<theta> \<tau>" and 
+    "w = worldline2 t \<sigma> \<theta> \<tau>" using destruct_worldline_exist worldline2_constructible by blast
+  moreover have "beval t \<sigma> \<gamma> \<theta> g"
+    using assms `w = worldline2 t \<sigma> \<theta> \<tau>` ci1  apply transfer' using beval_beval_world_ci by metis
+  ultimately have "t, \<sigma>, \<gamma>, \<theta> \<turnstile> <ss1, \<tau>> \<longrightarrow>\<^sub>s \<tau>'"
+    by auto
+  thus ?thesis
+    by (metis (no_types, lifting) \<open>t , \<sigma> , \<gamma> , \<theta> \<turnstile> <Bguarded g ss1 ss2 , \<tau>> \<longrightarrow>\<^sub>s \<tau>'\<close> case_prod_conv 
+        des1 world_seq_exec_def)
+qed
+
+lemma world_seq_exec_guarded_not:
+  assumes "\<not> beval_world2 w t g"
+  shows "world_seq_exec w t (Bguarded g ss1 ss2) = world_seq_exec w t ss2"
+proof -
+  obtain \<sigma> \<gamma> \<theta> \<tau> \<tau>' where des1: "destruct_worldline w t = (\<sigma>, \<gamma>, \<theta>, \<tau>)" and 
+    "t, \<sigma>, \<gamma>, \<theta> \<turnstile> <Bguarded g ss1 ss2, \<tau>> \<longrightarrow>\<^sub>s \<tau>'" and ci1: "context_invariant t \<sigma> \<gamma> \<theta> \<tau>" and 
+    "w = worldline2 t \<sigma> \<theta> \<tau>" using destruct_worldline_exist worldline2_constructible by blast
+  moreover have "\<not> beval t \<sigma> \<gamma> \<theta> g"
+    using assms `w = worldline2 t \<sigma> \<theta> \<tau>` ci1  apply transfer' using beval_beval_world_ci by metis
+  ultimately have "t, \<sigma>, \<gamma>, \<theta> \<turnstile> <ss2, \<tau>> \<longrightarrow>\<^sub>s \<tau>'"
+    by auto
+  thus ?thesis
+    by (metis (no_types, lifting) \<open>t , \<sigma> , \<gamma> , \<theta> \<turnstile> <Bguarded g ss1 ss2 , \<tau>> \<longrightarrow>\<^sub>s \<tau>'\<close> case_prod_conv 
+        des1 world_seq_exec_def)
+qed
+
+definition wp :: "'signal seq_stmt \<Rightarrow> nat \<Rightarrow> 'signal assn2 \<Rightarrow> 'signal assn2" where
+  "wp ss t Q = (\<lambda>w. \<forall>w'. (w, t, ss \<Rightarrow>\<^sub>s w') \<longrightarrow> Q w')"
+
+lemma wp_bnull: 
+  "wp Bnull t Q = Q"
+  by (rule ext)(auto simp add: wp_def world_seq_exec_bnull)
+
+lemma wp_bcomp:
+  "nonneg_delay (Bcomp ss1 ss2) \<Longrightarrow> wp (Bcomp ss1 ss2) t Q = wp ss1 t (wp ss2 t Q)"
+  by (rule ext) (auto simp add: wp_def world_seq_exec_comp)
+
+lemma wp_guarded: 
+  "wp (Bguarded g ss1 ss2) t Q = 
+  (\<lambda>w. if beval_world2 w t g then wp ss1 t Q w else wp ss2 t Q w)"
+  by (rule ext) (auto simp add: wp_def world_seq_exec_guarded world_seq_exec_guarded_not)
+
+lemma wp_trans: 
+  "wp (Bassign_trans sig exp dly) t Q = 
+  (\<lambda>w. Q(w[sig, t + dly :=\<^sub>2 beval_world2 w t exp]))"
+  by (rule ext, metis VHDL_Hoare_Complete.wp_def lift_world_trans_worldline_upd2)
+
+lemma wp_inert: 
+  "0 < dly \<Longrightarrow> wp (Bassign_inert sig exp dly) t Q = 
+  (\<lambda>w. Q(w[sig, t, dly :=\<^sub>2 beval_world2 w t exp]))"
+  by (rule ext, metis VHDL_Hoare_Complete.wp_def lift_world_inert_worldline_upd2) 
+
+lemma wp_is_pre: "nonneg_delay ss \<Longrightarrow> \<turnstile>\<^sub>t [wp ss t Q] ss [Q]"
+proof (induction ss arbitrary: Q)
+case (Bcomp ss1 ss2)
+  then show ?case by (auto simp add: wp_bcomp)
+next
+  case (Bguarded x1 ss1 ss2)
+  then show ?case by (auto intro:Conseq2 simp add: wp_guarded)
+next
+  case (Bassign_trans x1 x2 x3)
+  then show ?case by (auto simp add: wp_trans)
+next
+  case (Bassign_inert x1 x2 x3)
+  moreover have "0 < x3" using Bassign_inert by auto
+  ultimately show ?case  using AssignI2 by (auto simp add: wp_inert)
+next
+  case Bnull
+  then show ?case by (auto simp add: wp_bnull)
+qed
+
+lemma hoare_complete:
+  assumes "nonneg_delay ss" assumes "\<Turnstile>\<^sub>t [P] ss [Q]" shows "\<turnstile>\<^sub>t [P] ss [Q]"
+proof (rule strengthen_pre_hoare2)
+  show "\<forall>w. P w \<longrightarrow> wp ss t Q w" using assms
+    by (auto simp add:  seq_hoare_valid2_def wp_def)
+  show " \<turnstile>\<^sub>t [VHDL_Hoare_Complete.wp ss t Q] ss [Q]"
+    using assms by (intro wp_is_pre)
+qed
+
+corollary hoare_sound_complete: 
+  assumes "nonneg_delay ss"
+  shows "\<turnstile>\<^sub>t [P] ss [Q] \<longleftrightarrow> \<Turnstile>\<^sub>t [P] ss [Q]"
+  using hoare_complete soundness_hoare2 assms by auto
+
+end
